storeU ftlr case done

theories/ftlr/StoreU.v
@@ -421,8 +421,8 @@ Section fundamental.
        | Some a1 =>
          if (a1 =? a0)%Z
          then match std W !! a1 with
-              | Some (Uninitialized _) => (<[a0:=Monotemporary]> W.1,W.2)
-              | Some (Static _) => (<[a0:=Temporary]> W.1,W.2)
+              | Some (Uninitialized _) => (<[a1:=Monotemporary]> W.1,W.2)
+              | Some (Static _) => (<[a1:=Temporary]> W.1,W.2)
               | _ => W
               end
          else W
@@ -431,12 +431,52 @@ Section fundamental.
      | None => W
      end.
 
+   Lemma new_worldU_pub W a0 pc_p pc_g pc_b pc_e pc_a r offs :
+     (∀ g z a, z_of_argument (<[PC:=inr (pc_p, pc_g, pc_b, pc_e, pc_a)]> r) offs = Some z ∧
+               (a0 + z)%a = Some a ∧
+               W.1 !! a = Some (Static g) → ∃ w, g = {[a:=w]} ) →
+     related_sts_pub_world W (new_worldU W a0 pc_p pc_g pc_b pc_e pc_a r offs).
+   Proof.
+     intros Hcond. 
+     unfold new_worldU.
+     destruct (z_of_argument (<[PC:=inr (pc_p, pc_g, pc_b, pc_e, pc_a)]> r) offs);
+       [|apply related_sts_pub_refl_world].
+     destruct (a0 + z)%a eqn:Hnext;[|apply related_sts_pub_refl_world].
+     destruct (a =? a0)%Z;[|apply related_sts_pub_refl_world].
+     destruct (std W !! a) eqn:Hsome;[|apply related_sts_pub_refl_world].
+     destruct r0;try apply related_sts_pub_refl_world. 
+     - destruct Hcond with g z a as [w ->];auto.
+       apply uninitialized_related_sts_pub_world in Hsome;auto.
+     - apply uninitialized_w_mono_related_sts_pub_world in Hsome;auto. 
+   Qed.
+
+   Definition new_state ρ :=
+     match ρ with
+     | Static _ => Temporary
+     | Uninitialized _ => Monotemporary
+     | _ => ρ
+     end. 
+
+   Lemma new_worldU_lookup W a0 pc_p pc_g pc_b pc_e pc_a r offs z a1 ρ :
+     z_of_argument (<[PC:=inr (pc_p, pc_g, pc_b, pc_e, pc_a)]> r) offs = Some z →
+     (a0 + z)%a = Some a1 →
+     W.1 !! a1 = Some ρ →
+     (a1 =? a0)%Z = true →
+     std (new_worldU W a0 pc_p pc_g pc_b pc_e pc_a r offs) !! a1 = Some (new_state ρ).
+   Proof.
+     intros Hzoff Hnext Hρ Hfalse.
+     unfold new_worldU. rewrite Hzoff Hnext Hfalse Hρ.
+     unfold new_state. destruct ρ;auto;
+     simplify_map_eq;auto. 
+   Qed.
+
   (* Note that we turn in all information that we might have on the monotonicity of the current PC value, so that in the proof of the ftlr case itself, we do not have to worry about whether the PC was written to or not when we close the last location pc_a in the region *)
    Lemma mem_map_recover_res:
     ∀ (W : WORLD) (r : Reg) (p' : Perm)
        (pc_w : Word) (r1 : RegName) (r2 offs : Z + RegName) (offz : Z) (p0 p'0 pc_p pc_p' : Perm)
-       (g0 pc_g : Locality) (b0 e0 a0 a1 pc_b pc_e pc_a : Addr) (mem0 : PermMem) (oldv storev : Word) (ρ : region_type),
-      word_of_argument (<[PC:=inr (pc_p, pc_g, pc_b, pc_e, pc_a)]> r) r2 = Some storev
+       (g0 pc_g : Locality) (b0 e0 a0 a1 pc_b pc_e pc_a : Addr) (mem0 : PermMem) (oldv storev : Word) (ρ : region_type)
+       (Hnotstatic : ∀ g, ρ ≠ Static g) (Hnotuninitialized : ∀ w, ρ ≠ Uninitialized w), 
+        word_of_argument (<[PC:=inr (pc_p, pc_g, pc_b, pc_e, pc_a)]> r) r2 = Some storev
       → z_of_argument (<[PC:=inr (pc_p, pc_g, pc_b, pc_e, pc_a)]> r) offs = Some offz (* necessary for successful store *)
       → (a0 + offz)%a = Some a1 (* necessary for successful store *)
       → (pc_p = RX ∨ pc_p = RWX ∨ pc_p = RWLX)
@@ -451,13 +491,15 @@ Section fundamental.
         -∗ ([∗ map] a0↦pw ∈ <[a1 := (p'0, storev)]> mem0, ∃ (p0 : Perm) (w0 : Word),
                ⌜pw = (p0, w0)⌝ ∗ a0 ↦ₐ[p0] w0)
         -∗ sts_full_world W
-        -∗ ∃ v, open_region pc_a (new_worldU W a0 pc_p pc_g pc_b pc_e pc_a r offs)
+        ={⊤}=∗ ∃ v, open_region pc_a (new_worldU W a0 pc_p pc_g pc_b pc_e pc_a r offs)
                             ∗ sts_full_world (new_worldU W a0 pc_p pc_g pc_b pc_e pc_a r offs)
                             ∗ pc_a ↦ₐ[pc_p'] v
                             ∗ ((fixpoint interp1) (new_worldU W a0 pc_p pc_g pc_b pc_e pc_a r offs)) v
-                            ∗ monotonicity_guarantees_region ρ pc_a v pc_p' interpC.
+                            ∗ monotonicity_guarantees_region ρ pc_a v pc_p' interpC
+                            ∗ ⌜related_sts_pub_world W (new_worldU W a0 pc_p pc_g pc_b pc_e pc_a r offs)⌝.
    Proof.
-    intros W r p' pc_w r1 r2 offs offz p0 p'0 pc_p pc_p' g0 pc_g b0 e0 a0 a1 pc_b pc_e pc_a mem0 oldv storev ρ Hwoa Hz Hnext Hpcperm Hras Hstdst Ha0.
+     intros W r p' pc_w r1 r2 offs offz p0 p'0 pc_p pc_p' g0 pc_g b0 e0 a0 a1 pc_b pc_e pc_a mem0 oldv storev ρ Hnotstatic Hnotuninitialized
+            Hwoa Hz Hnext Hpcperm Hras Hstdst Ha0.
     iIntros "HStoreMem #Hreg #HVPCr #Hpc_w Hpcmono Hmem Hsts".
     iDestruct "HStoreMem" as (p1 g1 b1 e1 a1' storev1) "[% [% HStoreRes] ]".
     destruct (store_inr_eq Hras H) as (<- & <- &<- &<- &<-).
@@ -480,7 +522,7 @@ Section fundamental.
           destruct (<[PC:=inr (pc_p, pc_g, pc_b, pc_e, pc_a)]> r !! r0) eqn:Hrr0; inversion Hwoa; clear Hwoa; subst w.
           destruct (decide (r0 = PC)).
           + subst r0. rewrite lookup_insert in Hrr0. by inversion Hrr0.
-          + iSpecialize ("Hreg" $! r0 n).  rewrite lookup_insert_ne in Hrr0; last congruence. by rewrite /RegLocate Hrr0.
+          + iSpecialize ("Hreg" $! r0 n). rewrite lookup_insert_ne in Hrr0; last congruence. by rewrite /RegLocate Hrr0.
       }
       case_decide as Haeq.
       + iExists pc_w.
@@ -489,993 +531,399 @@ Section fundamental.
         rewrite lookup_insert in Ha0; inversion Ha0; clear Ha0; subst.
         iDestruct "HLoadRes" as (ρ1) "(Hstate' & % & % & % & % & % & Hr & % & Hrel')".
         rewrite insert_insert memMap_resource_2ne; last auto. iDestruct "Hmem" as  "[Ha1 $]".
-        iDestruct (storev_interp_mono with "HVr1") as "Hr1Mono";eauto.
-        destruct ((a1 =? a0)%Z) eqn:Heqa. apply Z.eqb_eq,z_of_eq in Heqa as ->.
-        * rewrite H1. admit. 
+        iDestruct (storev_interp_mono with "HVr1") as "Hr1Mono"; eauto.
+        destruct ((a1 =? a0)%Z) eqn:Heqa.
+        assert (related_sts_pub_world W (new_worldU W a0 pc_p pc_g pc_b pc_e pc_a r offs)) as Hpub.
+        { apply new_worldU_pub.
+          intros. destruct H7 as (?&?&?). simplify_eq. rewrite H1 in H9. inversion H9. eauto. }
+        iDestruct (storev_interp_mono (new_worldU W a0 pc_p pc_g pc_b pc_e pc_a r offs) with "[HVr1]") as "Hr1Mono2";
+          [eauto..|eapply new_worldU_lookup;eauto| |].
+        { iApply interp_monotone;[|iFrame "#"]. iPureIntro. auto. }
+        iDestruct (interp_monotone with "[] Hpc_w") as "Hpc_w'";[iPureIntro;apply Hpub|]. 
+        apply Z.eqb_eq,z_of_eq in Heqa as ->.
+        * rewrite H1. iFrame.
+          destruct (decide (ρ1 = Temporary ∨ ρ1 = Monotemporary ∨ ρ1 = Permanent)). 
+          ** iDestruct (region_close_next with "[$Hr $Ha1 $Hrel' $Hstate' $HVstorev1 $Hr1Mono]") as "Hr"; eauto;
+               [intros [g Hcontr];destruct o as [o |[o | o] ]; subst;try done..| |].
+             { apply not_elem_of_cons; split; [auto|apply not_elem_of_nil]. }
+             destruct o as [-> |[-> | ->] ]; iDestruct (region_open_prepare with "Hr") as "$"; iFrame; iFrame "Hpc_w";
+             iPureIntro;apply related_sts_pub_refl_world. 
+          ** apply Decidable.not_or in n as [Hne1 n].
+             apply Decidable.not_or in n as [Hne2 Hne3].
+             destruct ρ1;try congruence.
+             { (* ρ1 = Static g *)
+               unfold monotonicity_guarantees_region.
+               iSimpl in "Hr1Mono2". edestruct H4 as [w ->];auto.
+               destruct (pwl p'0) eqn:Hpwl. 
+               - iMod (region_close_next_uninit_pwl with "[$Hr $Hsts $Ha1 $Hrel' $Hstate' $HVstorev1 $Hr1Mono2]") as "[Hr Hsts]";eauto.
+                 { apply not_elem_of_cons; split; [auto|apply not_elem_of_nil]. }
+                 iModIntro. iDestruct (region_open_prepare with "Hr") as "$". iFrame. unfold new_worldU.
+                 rewrite Hz Hnext H1 Z.eqb_refl. iFrame "Hpc_w'".
+                 rewrite /new_worldU Hz Hnext H1 Z.eqb_refl in Hpub. auto. 
+               - iMod (region_close_next_uninit_nwl with "[$Hr $Hsts $Ha1 $Hrel' $Hstate' $HVstorev1 $Hr1Mono2]") as "[Hr Hsts]";eauto.
+                 { apply not_elem_of_cons; split; [auto|apply not_elem_of_nil]. }
+                 iModIntro. iDestruct (region_open_prepare with "Hr") as "$". iFrame. unfold new_worldU.
+                 rewrite Hz Hnext H1 Z.eqb_refl. iFrame "Hpc_w'".
+                 rewrite /new_worldU Hz Hnext H1 Z.eqb_refl in Hpub. auto.
+             }
+             { (* ρ1 = Uninitialized w *)
+               unfold monotonicity_guarantees_region.
+               iSimpl in "Hr1Mono2". 
+               destruct (pwl p'0) eqn:Hpwl. 
+               - iMod (region_close_next_mono_uninit_w_pwl with "[$Hr $Hsts $Ha1 $Hrel' $Hstate' $HVstorev1 $Hr1Mono2]") as "[Hr Hsts]";eauto.
+                 { apply not_elem_of_cons; split; [auto|apply not_elem_of_nil]. }
+                 iModIntro. iDestruct (region_open_prepare with "Hr") as "$". iFrame. unfold new_worldU.
+                 rewrite Hz Hnext H1 Z.eqb_refl. iFrame "Hpc_w'".
+                 rewrite /new_worldU Hz Hnext H1 Z.eqb_refl in Hpub. auto.
+               - iMod (region_close_next_mono_uninit_w_nwl with "[$Hr $Hsts $Ha1 $Hrel' $Hstate' $HVstorev1 $Hr1Mono2]") as "[Hr Hsts]";eauto.
+                 { apply not_elem_of_cons; split; [auto|apply not_elem_of_nil]. }
+                 iModIntro. iDestruct (region_open_prepare with "Hr") as "$". iFrame. unfold new_worldU.
+                 rewrite Hz Hnext H1 Z.eqb_refl. iFrame "Hpc_w'".
+                 rewrite /new_worldU Hz Hnext H1 Z.eqb_refl in Hpub. auto.
+             }
         * destruct H5 as [? ?].
           iDestruct (region_close_next with "[$Hr $Ha1 $Hrel' $Hstate' $HVstorev1 $Hr1Mono]") as "Hr"; eauto.
           { intros [g Hcontr]. specialize (H5 g). done. }
           { intros [g Hcontr]. specialize (H3 g). done. }
           { intros [g Hcontr]. specialize (H7 g). done. }
           { apply not_elem_of_cons; split; [auto|apply not_elem_of_nil]. }
-          iDestruct (region_open_prepare with "Hr") as "$". by iFrame.
+          iDestruct (region_open_prepare with "Hr") as "$". iFrame. iFrame "Hpc_w".
+          iPureIntro. apply related_sts_pub_refl_world. 
       + subst a1. iDestruct "HStoreRes" as "[-> [HStoreRes % ] ]".
         rewrite insert_insert -memMap_resource_1.
         rewrite lookup_insert in Ha0; inversion Ha0; simplify_eq.
         iExists storev1. iFrame.
+        rewrite Hstdst. 
         iDestruct (storev_interp_mono with "HVr1") as "Hr1Mono"; eauto.
+        destruct (pc_a =? a0)%Z eqn:Heqa0.
+        * destruct ρ; iFrame "∗ #"; try by (iPureIntro;apply related_sts_pub_refl_world).
+          exfalso. specialize (Hnotstatic g);done.
+          exfalso. specialize (Hnotuninitialized w);done. 
+        * iModIntro. iFrame "∗ #". iPureIntro. apply related_sts_pub_refl_world. 
     - by exfalso.
    Qed.
 
+   (* core lemma which will state that incrementing the address remains valid if world is initialized *)
+   Lemma interp_initialize_limit W a' x x0 x1 x2 x3 r offs p0 g0 b0 e0 a0 zoffs w0 r1:
+     related_sts_pub_world W (new_worldU W a' x x0 x1 x2 x3 r offs) →
+     z_of_argument (<[PC:=inr (x, x0, x1, x2, x3)]> r) offs = Some zoffs →
+     reg_allows_storeU (<[PC:=inr (x, x0, x1, x2, x3)]> r) r1 p0 g0 b0 e0 a' a' w0 →
+     (a' + zoffs)%a = Some a' →
+     (a' + 1)%a = Some a0 →
+     fixpoint interp1 W (inr (p0, g0, b0, e0, a')) -∗
+     fixpoint interp1 (new_worldU W a' x x0 x1 x2 x3 r offs) (inr (p0, g0, b0, e0, a0)).
+   Proof.
+     iIntros (Hpub Hzoff Hallows Ha' Hnext) "#Hvalid".
+     destruct Hallows as [Hlookup [Hu (Hle1 & Hle2 & Hle3 & Hallows)] ].
+     iDestruct (interp_monotone with "[] Hvalid") as "Hvalid'";[eauto|].
+     iClear "Hvalid".
+     destruct p0;inversion Hu;rewrite !fixpoint_interp1_eq /=;eauto.
+     - destruct g0;try done.
+       + iDestruct "Hvalid'" as "[Hval1 Hval2]".
+         assert (addr_reg.min a' e0 <= addr_reg.min a0 e0)%Z;[solve_addr|].
+         assert (b0 <= (addr_reg.min a' e0))%Z;[solve_addr|].
+         rewrite (region_addrs_split b0 (addr_reg.min a' e0) (addr_reg.min a0 e0));[|solve_addr].
+         rewrite big_sepL_app. rewrite bi.sep_comm. iFrame "Hval1".
+         assert (addr_reg.max b0 a0 <= e0)%a;[solve_addr|].
+         rewrite (region_addrs_split (addr_reg.max b0 a') (addr_reg.max b0 a0) e0);[|solve_addr].
+         iDestruct (big_sepL_app with "Hval2") as "[Hval21 Hval22]". iFrame "Hval22".
+         assert (addr_reg.min a' e0 = a') as ->;[solve_addr|].
+         assert (addr_reg.min a0 e0 = a0) as ->;[solve_addr|].
+         assert (addr_reg.max b0 a' = a') as ->;[solve_addr|].
+         assert (addr_reg.max b0 a0 = a0) as ->;[solve_addr|].
+         rewrite (region_addrs_single a' a0);auto. simpl.
+         iDestruct "Hval21" as "[Hval21 _]".
+         iDestruct "Hval21" as (p0 Hflows) "[Hrel %]".
+         iSplit;auto. iExists p0. repeat iSplit;auto. iPureIntro.
 
+         unfold region_state_U in H0. destruct H2 as [-> | [-> | [w Hstatic] ] ];auto.
+         unfold new_worldU in Hstatic. rewrite Hzoff Ha' Z.eqb_refl in Hstatic.
+         unfold new_worldU. rewrite Hzoff Ha' Z.eqb_refl.
+         destruct (std W !! a') eqn:Hsome;[|congruence]. 
+         destruct r0;inversion Hstatic; try congruence.
+         simplify_map_eq. simplify_map_eq.
+       + iDestruct "Hvalid'" as "[Hval1 Hval2]".
+         assert (addr_reg.min a' e0 <= addr_reg.min a0 e0)%Z;[solve_addr|].
+         assert (b0 <= (addr_reg.min a' e0))%Z;[solve_addr|].
+         rewrite (region_addrs_split b0 (addr_reg.min a' e0) (addr_reg.min a0 e0));[|solve_addr].
+         rewrite big_sepL_app. rewrite bi.sep_comm. iFrame "Hval1".
+         assert (addr_reg.max b0 a0 <= e0)%a;[solve_addr|].
+         rewrite (region_addrs_split (addr_reg.max b0 a') (addr_reg.max b0 a0) e0);[|solve_addr].
+         iDestruct (big_sepL_app with "Hval2") as "[Hval21 Hval22]". iFrame "Hval22".
+         assert (addr_reg.min a' e0 = a') as ->;[solve_addr|].
+         assert (addr_reg.min a0 e0 = a0) as ->;[solve_addr|].
+         assert (addr_reg.max b0 a' = a') as ->;[solve_addr|].
+         assert (addr_reg.max b0 a0 = a0) as ->;[solve_addr|].
+         rewrite (region_addrs_single a' a0);auto. simpl.
+         iDestruct "Hval21" as "[Hval21 _]".
+         iDestruct "Hval21" as (p0 Hflows) "[Hrel %]".
+         iSplit;auto. iExists p0. repeat iSplit;auto. iPureIntro.
 
+         unfold region_state_U in H0. destruct H2 as [-> | [-> | [ -> | [ [w Hstatic] | [w Hstatic] ] ] ] ];auto.
+         all: unfold new_worldU in Hstatic;rewrite Hzoff Ha' Z.eqb_refl in Hstatic.
+         all: unfold new_worldU;rewrite Hzoff Ha' Z.eqb_refl.
+         all: destruct (std W !! a') eqn:Hsome;[|congruence]. 
+         all: destruct r0;inversion Hstatic; try congruence.
+         all: simplify_map_eq. 
+     - destruct g0;try done.
+       iDestruct "Hvalid'" as "[Hval1 Hval2]".
+       assert (addr_reg.min a' e0 <= addr_reg.min a0 e0)%Z;[solve_addr|].
+       assert (b0 <= (addr_reg.min a' e0))%Z;[solve_addr|].
+       rewrite (region_addrs_split b0 (addr_reg.min a' e0) (addr_reg.min a0 e0));[|solve_addr].
+       rewrite big_sepL_app. rewrite bi.sep_comm. iFrame "Hval1".
+       assert (addr_reg.max b0 a0 <= e0)%a;[solve_addr|].
+       rewrite (region_addrs_split (addr_reg.max b0 a') (addr_reg.max b0 a0) e0);[|solve_addr].
+       iDestruct (big_sepL_app with "Hval2") as "[Hval21 Hval22]". iFrame "Hval22".
+       assert (addr_reg.min a' e0 = a') as ->;[solve_addr|].
+       assert (addr_reg.min a0 e0 = a0) as ->;[solve_addr|].
+       assert (addr_reg.max b0 a' = a') as ->;[solve_addr|].
+       assert (addr_reg.max b0 a0 = a0) as ->;[solve_addr|].
+       rewrite (region_addrs_single a' a0);auto. simpl.
+       iDestruct "Hval21" as "[Hval21 _]".
+       iDestruct "Hval21" as (p0 Hflows) "[Hrel %]".
+       iSplit;auto. iExists p0. repeat iSplit;auto. iPureIntro.
 
+       unfold region_state_U in H0. destruct H2 as [Hw | [w Hstatic] ];auto.
+       unfold new_worldU in Hstatic. rewrite Hzoff Ha' Z.eqb_refl in Hstatic.
+       unfold new_worldU. rewrite Hzoff Ha' Z.eqb_refl.
+       destruct (std W !! a') eqn:Hsome;[|congruence]. 
+       destruct r0;inversion Hstatic; try congruence.
+       simplify_map_eq. simplify_map_eq.
+     - destruct g0;try done.
+       + iDestruct "Hvalid'" as "[Hval1 Hval2]".
+         assert (addr_reg.min a' e0 <= addr_reg.min a0 e0)%Z;[solve_addr|].
+         assert (b0 <= (addr_reg.min a' e0))%Z;[solve_addr|].
+         rewrite (region_addrs_split b0 (addr_reg.min a' e0) (addr_reg.min a0 e0));[|solve_addr].
+         rewrite big_sepL_app. rewrite bi.sep_comm. iFrame "Hval1".
+         assert (addr_reg.max b0 a0 <= e0)%a;[solve_addr|].
+         rewrite (region_addrs_split (addr_reg.max b0 a') (addr_reg.max b0 a0) e0);[|solve_addr].
+         iDestruct (big_sepL_app with "Hval2") as "[Hval21 Hval22]". iFrame "Hval22".
+         assert (addr_reg.min a' e0 = a') as ->;[solve_addr|].
+         assert (addr_reg.min a0 e0 = a0) as ->;[solve_addr|].
+         assert (addr_reg.max b0 a' = a') as ->;[solve_addr|].
+         assert (addr_reg.max b0 a0 = a0) as ->;[solve_addr|].
+         rewrite (region_addrs_single a' a0);auto. simpl.
+         iDestruct "Hval21" as "[Hval21 _]".
+         iDestruct "Hval21" as (p0 Hflows) "[Hrel %]".
+         iSplit;auto. iExists p0. repeat iSplit;auto. iPureIntro.
 
+         unfold region_state_U in H0. destruct H2 as [-> | [-> | [w Hstatic] ] ];auto.
+         unfold new_worldU in Hstatic. rewrite Hzoff Ha' Z.eqb_refl in Hstatic.
+         unfold new_worldU. rewrite Hzoff Ha' Z.eqb_refl.
+         destruct (std W !! a') eqn:Hsome;[|congruence]. 
+         destruct r0;inversion Hstatic; try congruence.
+         simplify_map_eq. simplify_map_eq.
+       + iDestruct "Hvalid'" as "[Hval1 Hval2]".
+         assert (addr_reg.min a' e0 <= addr_reg.min a0 e0)%Z;[solve_addr|].
+         assert (b0 <= (addr_reg.min a' e0))%Z;[solve_addr|].
+         rewrite (region_addrs_split b0 (addr_reg.min a' e0) (addr_reg.min a0 e0));[|solve_addr].
+         rewrite big_sepL_app. rewrite bi.sep_comm. iFrame "Hval1".
+         assert (addr_reg.max b0 a0 <= e0)%a;[solve_addr|].
+         rewrite (region_addrs_split (addr_reg.max b0 a') (addr_reg.max b0 a0) e0);[|solve_addr].
+         iDestruct (big_sepL_app with "Hval2") as "[Hval21 Hval22]". iFrame "Hval22".
+         assert (addr_reg.min a' e0 = a') as ->;[solve_addr|].
+         assert (addr_reg.min a0 e0 = a0) as ->;[solve_addr|].
+         assert (addr_reg.max b0 a' = a') as ->;[solve_addr|].
+         assert (addr_reg.max b0 a0 = a0) as ->;[solve_addr|].
+         rewrite (region_addrs_single a' a0);auto. simpl.
+         iDestruct "Hval21" as "[Hval21 _]".
+         iDestruct "Hval21" as (p0 Hflows) "[Hrel %]".
+         iSplit;auto. iExists p0. repeat iSplit;auto. iPureIntro.
 
+         unfold region_state_U in H0. destruct H2 as [-> | [-> | [ -> | [ [w Hstatic] | [w Hstatic] ] ] ] ];auto.
+         all: unfold new_worldU in Hstatic;rewrite Hzoff Ha' Z.eqb_refl in Hstatic.
+         all: unfold new_worldU;rewrite Hzoff Ha' Z.eqb_refl.
+         all: destruct (std W !! a') eqn:Hsome;[|congruence]. 
+         all: destruct r0;inversion Hstatic; try congruence.
+         all: simplify_map_eq.
+     - destruct g0;try done.
+       iDestruct "Hvalid'" as "[Hval1 Hval2]".
+       assert (addr_reg.min a' e0 <= addr_reg.min a0 e0)%Z;[solve_addr|].
+       assert (b0 <= (addr_reg.min a' e0))%Z;[solve_addr|].
+       rewrite (region_addrs_split b0 (addr_reg.min a' e0) (addr_reg.min a0 e0));[|solve_addr].
+       rewrite big_sepL_app. rewrite bi.sep_comm. iFrame "Hval1".
+       assert (addr_reg.max b0 a0 <= e0)%a;[solve_addr|].
+       rewrite (region_addrs_split (addr_reg.max b0 a') (addr_reg.max b0 a0) e0);[|solve_addr].
+       iDestruct (big_sepL_app with "Hval2") as "[Hval21 Hval22]". iFrame "Hval22".
+       assert (addr_reg.min a' e0 = a') as ->;[solve_addr|].
+       assert (addr_reg.min a0 e0 = a0) as ->;[solve_addr|].
+       assert (addr_reg.max b0 a' = a') as ->;[solve_addr|].
+       assert (addr_reg.max b0 a0 = a0) as ->;[solve_addr|].
+       rewrite (region_addrs_single a' a0);auto. simpl.
+       iDestruct "Hval21" as "[Hval21 _]".
+       iDestruct "Hval21" as (p0 Hflows) "[Hrel %]".
+       iSplit;auto. iExists p0. repeat iSplit;auto. iPureIntro.
 
+       unfold region_state_U in H0. destruct H2 as [Hw | [w Hstatic] ];auto.
+       unfold new_worldU in Hstatic. rewrite Hzoff Ha' Z.eqb_refl in Hstatic.
+       unfold new_worldU. rewrite Hzoff Ha' Z.eqb_refl.
+       destruct (std W !! a') eqn:Hsome;[|congruence]. 
+       destruct r0;inversion Hstatic; try congruence.
+       simplify_map_eq. simplify_map_eq.
+   Qed. 
 
-
-
-
-
-
-
-  (* TODO: move somewhere *)
-  Lemma isU_inv:
-    ∀ (W : leibnizO WORLD) (a' a b e : Addr) (p : Perm) (g : Locality),
-      (b ≤ a' < addr_reg.min a e)%Z
-      → isU p = true
-      → ⊢ (interp W) (inr (p, g, b, e, a))
-      → ∃ p' : Perm, ⌜PermFlows (promote_perm p) p'⌝ ∗ read_write_cond a' p' interp
-                     ∧ ⌜(∃ ρ : region_type, std W !! a' = Some ρ
-                                            ∧ ρ ≠ Revoked /\ (∀ g, ρ ≠ Static g) ∧ (∀ g, ρ ≠ Monostatic g) ∧ (∀ w, ρ ≠ Uninitialized w))⌝.
-  Proof.
-    intros. rewrite /interp fixpoint_interp1_eq /=. iIntros "H".
-    assert (p = URW \/ p = URWL \/ p = URWX \/ p = URWLX) as [-> | [-> | [-> | ->] ] ] by (destruct p; simpl in H0; auto; congruence); simpl.
-    - destruct g.
-      + iDestruct (extract_from_region_inv with "H") as (p' ?) "[C %]";try (iExists p'; iFrame; auto);[solve_addr|].
-        iSplit;auto. iPureIntro; auto. rewrite H2. eexists;eauto.
-      + iDestruct "H" as "[B C]".
-        iDestruct (extract_from_region_inv with "B") as (p' ?) "[D %]"; try (iExists p'; iFrame); auto.
-        iSplit;auto. iPureIntro; auto. destruct H2; eexists;eauto.
-      + iDestruct "H" as "[B C]".
-        iDestruct (extract_from_region_inv with "B") as (p' ?) "[D %]"; try (iExists p'; iFrame); auto.
-        iSplit;auto. iPureIntro; auto. destruct H2 as [? | [? | ?] ]; eexists;eauto.
-    - destruct g; auto.
-      iDestruct "H" as "[B C]".
-      iDestruct (extract_from_region_inv with "B") as (p' ?) "[D %]"; try (iExists p'; iFrame); auto.
-      iPureIntro; split;eauto. eexists;eauto.
-    - destruct g.
-      + iDestruct (extract_from_region_inv with "H") as (p' Hfl) "[D %]"; try (iExists p'; iFrame); auto; [solve_addr|].
-        iSplit;auto. iPureIntro; auto. eexists; eauto.
-      + iDestruct "H" as "[B C]".
-        iDestruct (extract_from_region_inv with "B") as (p' Hfl) "[E %]"; try (iExists p'; iFrame); auto.
-        iSplit;auto. iPureIntro; auto. destruct H1; eexists;eauto.
-      + iDestruct "H" as "[B C]".
-        iDestruct (extract_from_region_inv with "B") as (p' Hfl) "[E %]"; try (iExists p'; iFrame); auto.
-        iSplit;auto. iPureIntro; auto. destruct H1 as [? | [? | ?] ]; eexists;eauto.
-    - destruct g; auto.
-      iDestruct "H" as "[B C]".
-      iDestruct (extract_from_region_inv with "B") as (p' Hfl) "[D %]"; try (iExists p'; iFrame); auto.
-      iSplit;auto. iPureIntro; simpl in H1; eexists;eauto.
-  Qed.
-
-  
-
-
-
-
-
-
-
-
-
-
-
-
-
-
-
-
-
-
-
-  (* Lemma region_open_next_perm' W ls l p : *)
-  (*   l ∉ ls → (std_sta W) !! (countable.encode l) = Some (countable.encode Permanent) ->  *)
-  (*   open_region_many ls W ∗ sts_full_world sts_std W ∗ uninitialized_cond l p -∗ *)
-  (*                    ∃ v, sts_full_world sts_std W *)
-  (*                         ∗ sts_state_std (countable.encode l) Permanent *)
-  (*                         ∗ open_region_many (l :: ls) W *)
-  (*                         ∗ l ↦ₐ[p] v *)
-  (*                         ∗ ⌜p ≠ O⌝. *)
-  (* Proof. *)
-  (*   rewrite open_region_many_eq .  *)
-  (*   iIntros (Hnin Htemp) "(Hopen & Hfull & Hun)". *)
-  (*   rewrite /open_region_many_def /= /region_map_def. *)
-  (*   rewrite /region_def /region. *)
-  (*   iDestruct "Hopen" as (M) "(HM & % & Hpreds)". *)
-  (*   destruct (proj1 (H3 (countable.encode l)) ltac:(eauto)) as [l' [X1 X2] ]. *)
-  (*   eapply encode_inj in X1; subst l'. destruct X2 as [γp HX]. *)
-  (*   iDestruct "Hun" as (γrel) "Hγpred". rewrite RELS_eq /RELS_def REL_eq /REL_def. *)
-  (*   iDestruct (reg_in with "[$HM $Hγpred]") as %HMeq. *)
-  (*   rewrite HMeq delete_list_insert; auto. *)
-  (*   rewrite delete_list_delete; auto. *)
-  (*   rewrite big_sepM_insert; [|by rewrite lookup_delete]. *)
-  (*   iDestruct "Hpreds" as "[Hl Hpreds]". *)
-  (*   iDestruct "Hl" as (ρ) "[Hstate Hl]". destruct ρ. *)
-  (*   1,3,4: iDestruct (sts_full_state_std with "Hfull Hstate") as %Hcontr. *)
-  (*   1,2,3: rewrite Htemp in Hcontr; inversion Hcontr; apply countable.encode_inj in H5; done.     iDestruct "Hl" as (γpred' v p' ϕ) "(% & % & Hl & HX & HY & HZ)". *)
-  (*   inversion H4; subst. *)
-  (*   iExists v. iFrame. *)
-  (*   iSplitL; auto. *)
-  (*   iExists _. iFrame "∗ #". rewrite <- HMeq. auto. *)
-  (* Qed. *)
-
-  (* Lemma region_open_next_temp' W ls l p : *)
-  (*   l ∉ ls → (std_sta W) !! (countable.encode l) = Some (countable.encode Temporary) ->  *)
-  (*   open_region_many ls W ∗ sts_full_world sts_std W ∗ uninitialized_cond l p -∗ *)
-  (*                    ∃ v, sts_full_world sts_std W *)
-  (*                         ∗ sts_state_std (countable.encode l) Temporary *)
-  (*                         ∗ open_region_many (l :: ls) W *)
-  (*                         ∗ l ↦ₐ[p] v *)
-  (*                         ∗ ⌜p ≠ O⌝. *)
-  (* Proof. *)
-  (*   rewrite open_region_many_eq .  *)
-  (*   iIntros (Hnin Htemp) "(Hopen & Hfull & Hun)". *)
-  (*   rewrite /open_region_many_def /= /region_map_def. *)
-  (*   rewrite /region_def /region. *)
-  (*   iDestruct "Hopen" as (M) "(HM & % & Hpreds)". *)
-  (*   destruct (proj1 (H3 (countable.encode l)) ltac:(eauto)) as [l' [X1 X2] ]. *)
-  (*   eapply encode_inj in X1; subst l'. destruct X2 as [γp HX]. *)
-  (*   iDestruct "Hun" as (γrel) "Hγpred". rewrite RELS_eq /RELS_def REL_eq /REL_def. *)
-  (*   iDestruct (reg_in with "[$HM $Hγpred]") as %HMeq. *)
-  (*   rewrite HMeq delete_list_insert; auto. *)
-  (*   rewrite delete_list_delete; auto. *)
-  (*   rewrite big_sepM_insert; [|by rewrite lookup_delete]. *)
-  (*   iDestruct "Hpreds" as "[Hl Hpreds]". *)
-  (*   iDestruct "Hl" as (ρ) "[Hstate Hl]". destruct ρ. *)
-  (*   2,3,4: iDestruct (sts_full_state_std with "Hfull Hstate") as %Hcontr. *)
-  (*   2,3,4: rewrite Htemp in Hcontr; inversion Hcontr; apply countable.encode_inj in H5; done.     iDestruct "Hl" as (γpred' v p' ϕ) "(% & % & Hl & HX & HY & HZ)". *)
-  (*   inversion H4; subst. *)
-  (*   iExists v. iFrame. *)
-  (*   iSplitL; auto. *)
-  (*   iExists _. iFrame "∗ #". rewrite <- HMeq. auto. *)
-  (* Qed. *)
-
-  Lemma region_open_next_uninit' W ls l p w :
-    l ∉ ls → (std W) !! l = Some (Static {[l:=w]}) ->
-    open_region_many ls W ∗ sts_full_world W ∗ read_write_cond l p interp -∗
-                            sts_full_world W
-                          ∗ sts_state_std l (Static {[l:=w]})
-                          ∗ open_region_many (l :: ls) W
-                          ∗ l ↦ₐ[p] w
-                          ∗ ⌜p ≠ O⌝.
-  Proof.
-    rewrite open_region_many_eq .
-    iIntros (Hnin Htemp) "(Hopen & Hfull & Hun)".
-    rewrite /open_region_many_def /= /region_map_def.
-    rewrite /region_def /region.
-    iDestruct "Hopen" as (M Mρ) "(HM & % & % & Hpreds)".
-    assert (is_Some (M !! l)) as [γp HX].
-    { apply elem_of_gmap_dom. rewrite -H. apply elem_of_gmap_dom. eauto. }
-    rewrite /read_write_cond rel_eq /rel_def.
-    iDestruct "Hun" as (γrel) "[Hγpred BB]". rewrite RELS_eq /RELS_def REL_eq /REL_def.
-    iDestruct (reg_in with "[$HM $Hγpred]") as %HMeq.
-    rewrite HMeq delete_list_insert; auto.
-    rewrite delete_list_delete; auto.
-    rewrite big_sepM_insert; [|by rewrite lookup_delete].
-    iDestruct "Hpreds" as "[Hl Hpreds]".
-    iDestruct "Hl" as (ρ) "[ % [Hstate Hl] ]". destruct ρ.
-    1,2,3,4: iDestruct (sts_full_state_std with "Hfull Hstate") as %Hcontr.
-    1,2,3,4: try (rewrite Htemp in Hcontr; by inversion Hcontr).
-    iDestruct "Hl" as (γpred p0 φ Heq Hpers) "[#Hsaved Hl]". inversion Heq.
-    iDestruct "Hl" as (v Hlookup Hneq) "[Hl _]". rewrite Htemp in Hcontr. inversion Hcontr. subst g.
-    rewrite lookup_insert in Hlookup. inversion Hlookup.
-    iFrame.
-    repeat iSplitL; auto.
-    iExists _,Mρ. iFrame "∗ #". subst. rewrite -HMeq.
-    repeat iSplit;auto.
-    iApply (region_map_delete_singleton with "Hpreds");eauto.
-  Qed.
-
-  Lemma region_open_next' W ls l ρ p:
-    ρ <> Revoked ∧ (forall m, ρ = Static m -> (∃ w, m = {[l:=w]})) ->
-    l ∉ ls → (std W) !! l = Some ρ ->
-    open_region_many ls W ∗ sts_full_world W ∗ read_write_cond l p interp -∗
-                     ∃ v, sts_full_world W
-                          ∗ sts_state_std l ρ
-                          ∗ open_region_many (l :: ls) W
-                          ∗ l ↦ₐ[p] v
-                          ∗ ⌜p ≠ O⌝.
-  Proof.
-    iIntros ([Hnotrevoked Hnotstatic] Hnotin Hstd) "[A [B C]]". destruct ρ; try congruence.
-    - destruct (pwl p) eqn:Hpwl.
-      + iDestruct (region_open_next_temp_pwl with "[$A $B $C]") as "X"; auto.
-        iDestruct "X" as (v) "[A [B [C [D [E F]]]]]".
-        iExists v. iFrame.
-      + iDestruct (region_open_next_temp_nwl with "[$A $B $C]") as "X"; auto.
-        iDestruct "X" as (v) "[A [B [C [D [E F]]]]]".
-        iExists v. iFrame.
-    - iDestruct (region_open_next_perm with "[$A $B $C]") as "X"; auto.
-      iDestruct "X" as (v) "[A [B [C [D [E F]]]]]".
-      iExists v. iFrame.
-    - destruct Hnotstatic with g as [w Hw];auto. subst g. iExists w.
-      iApply region_open_next_uninit'; eauto; iFrame.
-  Qed.
-
-  Lemma isU_limit_inv:
-    ∀ (W : leibnizO WORLD) (a b e : Addr) (p : Perm) (g : Locality),
-      (b ≤ a < e)%Z ->
-      isU p = true ->
-      (interp W) (inr (p, g, b, e, a)) -∗
-      ∃ p' : Perm,
-        ⌜PermFlows (promote_perm p) p'⌝ ∗
-         read_write_cond a p' interp ∧
-        ⌜(∃ ρ : region_type, std W !! a = Some ρ
-                             ∧ ρ ≠ Revoked ∧ (forall m, ρ = Static m -> (∃ w, m = {[a:=w]})))⌝.
-  Proof.
-    intros. rewrite /interp fixpoint_interp1_eq /=. iIntros "H".
-    assert (p = URW \/ p = URWL \/ p = URWX \/ p = URWLX) as [-> | [-> | [-> | ->] ] ] by (destruct p; simpl in H0; auto; congruence); simpl.
-    - destruct g.
-      + iDestruct (extract_from_region_inv with "H") as (p' ?) "[C %]"; eauto.
-        iExists p'. iSplit;auto. simpl. iFrame. iPureIntro. eexists. repeat split;eauto. done.
-      + iDestruct "H" as "[B C]".
-        iDestruct (extract_from_region_inv with "C") as (p' ?) "[D %]"; try (iExists p'; iSplit;auto;iFrame); eauto.
-        split;auto;solve_addr.
-        iPureIntro; destruct H2 as [-> | [-> | [ ? -> ] ] ]; eexists;repeat split;eauto; try done.
-        intros m Hm. inversion Hm. exists x. auto.
-    - destruct g; auto.
-      iDestruct "H" as "[B C]".
-      iDestruct (extract_from_region_inv with "C") as (p' ?) "[D %]"; try (iExists p'; iSplit;auto;iFrame); eauto.
-      split; eauto; solve_addr.
-      iPureIntro; eauto. destruct H2 as [-> | [? ->] ]; eexists;repeat split;eauto;try done.
-      intros m Hm; inversion Hm. eauto.
-    - destruct g.
-      + iDestruct (extract_from_region_inv with "H") as (p' ?) "[D %]"; try (iExists p'; iSplit;auto;iFrame);auto.
-        iPureIntro. eexists;repeat split;eauto; try done.
-      + iDestruct "H" as "[B C]".
-        iDestruct (extract_from_region_inv with "C") as (p' ?) "[E %]"; try (iExists p'; iSplit;auto;iFrame);auto.
-        split; eauto; solve_addr.
-        iPureIntro; auto. destruct H2 as [-> | [-> | [? ->] ] ]; eexists;repeat split;eauto; try done.
-        intros m Hm; inversion Hm;eauto.
-    - destruct g; auto.
-      iDestruct "H" as "[B D]".
-      iDestruct (extract_from_region_inv with "D") as (p' ?) "[E %]"; try (iExists p'; iSplit;auto;iFrame); eauto.
-      split; eauto; solve_addr.
-      iPureIntro; auto. destruct H2 as [-> | [? ->] ]; eexists;repeat split;eauto; try done.
-      intros m Hm; inversion Hm;eauto.
-  Qed.
-
-  Definition region_open_resources W l ls p φ v (bl : bool): iProp Σ :=
-    (∃ ρ,
-     sts_state_std l ρ
-    ∗ ⌜ρ ≠ Revoked ∧ (forall m, ρ ≠ Static m)⌝
-    ∗ open_region_many (l :: ls) W
-    ∗ ⌜p ≠ O⌝
-    ∗ (if bl then monotonicity_guarantees_region ρ v p φ ∗ φ (W, v)
-       else ▷ monotonicity_guarantees_region ρ v p φ ∗  ▷ φ (W, v) )
-    ∗ rel l p φ)%I.
-
-  Definition region_open_resources_uninit W l ls p (bl : bool): iProp Σ :=
-    (∃ ρ,
-     sts_state_std l ρ
-    ∗ ⌜ρ ≠ Revoked ∧ (forall m, ρ = Static m -> (∃ w, m = {[l:=w]}))⌝
-    ∗ open_region_many (l :: ls) W
-    ∗ ⌜p ≠ O⌝
-    ∗ read_write_cond l p interp)%I.
-
-  (* TODO: move upstream to Iris ?*)
-  Instance if_persistent {PROP:bi} P Q (b: bool):
-    Persistent P ->
-    Persistent Q ->
-    Persistent (PROP := PROP) (if b then P else Q).
-  Proof.
-    intros; destruct b; auto.
-  Qed.
-
-  (* TODO: move into logrel.v *)
-  (* Quality of life lemma *)
-  Global Instance future_world_pure g W W':
-    IntoPure (@future_world Σ g W W')
-             (match g with Global => related_sts_priv_world W W' | Local => related_sts_pub_world W W' end).
-  Proof. red; intros. destruct g; auto. Qed.
-
-  Lemma region_close_next_uninit_pwl W ls l φ p w v `{forall Wv, Persistent (φ Wv)}:
-    l ∉ ls ->
-    pwl p = true →
-    sts_state_std l (Static {[l:=w]})
-    ∗ open_region_many (l::ls) W
-    ∗ l ↦ₐ[p] v
-    ∗ ⌜p ≠ O⌝
-    ∗ future_pub_mono φ v
-    ∗ ▷ φ (W,v) (* Maybe φ (<l[ l := Temporary, (Rpub, Rpriv) ]l> W, v) *)
-    ∗ rel l p φ
-    ∗ sts_full_world W
-    ==∗ open_region_many ls (<s[ l := Temporary ]s> W) ∗ sts_full_world (<s[ l := Temporary ]s> W).
-  Proof.
-    rewrite open_region_many_eq rel_eq /open_region_many_def /rel_def /region_def
-            REL_eq RELS_eq /RELS_def /REL_def.
-    iIntros (Hnin Hpwl) "(Hstate & Hreg_open & Hl & % & #Hmono & Hφ & #Hrel & Hfull)".
-    iDestruct "Hrel" as (γpred) "#[Hγpred Hφ_saved]".
-    iDestruct "Hreg_open" as (M Mρ) "(HM & % & % & Hpreds)".
-    iDestruct (sts_full_state_std with "Hfull Hstate") as "%".
-    iDestruct (sts_update_std with "Hfull Hstate") as ">[Hfull Hstate]".
-    iDestruct (reg_in γrel M with "[$HM $Hγpred]") as %HMeq.
-    iModIntro. iSplitR "Hfull".
-    { iDestruct (big_sepM_insert _ (delete l (delete_list ls M)) l with "[-HM]") as "Hmap_def";
-        first by rewrite lookup_delete.
-      { simpl.
-        iDestruct (region_map_insert_nonstatic Temporary with "Hpreds") as "Hpreds";auto.
-        iFrame. iExists Temporary. iFrame.
-        iSplit;[iPureIntro;apply lookup_insert|].
-        iExists γpred, p, _. iFrame "∗ #". repeat iSplitR; auto.
-        iExists v. rewrite Hpwl. auto. }
-      assert (Hpub: related_sts_pub_world W (<s[l:=Temporary]s>W)).
-      { eapply (uninitialized_related_sts_pub_world l W); eauto. }
-      iDestruct (region_map_monotone _ _ _ _ Hpub with "Hmap_def") as "HMdef"; eauto.
-      iExists M,(<[l:=Temporary]>Mρ); iFrame.
-      assert (l ∈ dom (gset Addr) M) as Hin.
-      { rewrite -H1. apply elem_of_gmap_dom. eauto. }
-      repeat rewrite dom_insert_L.
-      repeat iSplit;[iPureIntro..|];[rewrite H1;set_solver|rewrite H2;set_solver|].
-      rewrite -delete_list_delete;auto. rewrite -delete_list_insert; auto. rewrite -HMeq.
-      rewrite delete_list_insert; auto. }
-    iFrame.
-  Qed.
-
-  Lemma region_close_next_uninit_nwl W ls l φ p w v `{forall Wv, Persistent (φ Wv)}:
-    l ∉ ls ->
-    pwl p = false →
-    sts_state_std l (Static {[l:=w]})
-    ∗ open_region_many (l::ls) W
-    ∗ l ↦ₐ[p] v
-    ∗ ⌜p ≠ O⌝
-    ∗ future_priv_mono φ v
-    ∗ ▷ φ (W,v) (* Maybe φ (<l[ l := Temporary, (Rpub, Rpriv) ]l> W, v) *)
-    ∗ rel l p φ
-    ∗ sts_full_world W
-    ==∗ open_region_many ls (<s[ l := Temporary ]s> W) ∗ sts_full_world (<s[ l := Temporary ]s> W).
-  Proof.
-    rewrite open_region_many_eq rel_eq /open_region_many_def /rel_def /region_def
-            REL_eq RELS_eq /RELS_def /REL_def.
-    iIntros (Hnin Hpwl) "(Hstate & Hreg_open & Hl & % & #Hmono & Hφ & #Hrel & Hfull)".
-    iDestruct "Hrel" as (γpred) "#[Hγpred Hφ_saved]".
-    iDestruct "Hreg_open" as (M Mρ) "(HM & % & % & Hpreds)".
-    iDestruct (sts_full_state_std with "Hfull Hstate") as "%".
-    iDestruct (sts_update_std with "Hfull Hstate") as ">[Hfull Hstate]".
-    iDestruct (reg_in γrel M with "[$HM $Hγpred]") as %HMeq.
-    iModIntro. iSplitR "Hfull".
-    { iDestruct (big_sepM_insert _ (delete l (delete_list ls M)) l with "[-HM]") as "Hmap_def";
-        first by rewrite lookup_delete.
-      { simpl.
-        iDestruct (region_map_insert_nonstatic Temporary with "Hpreds") as "Hpreds";auto.
-        iFrame. iExists Temporary. iFrame.
-        iSplit;[iPureIntro;apply lookup_insert|].
-        iExists γpred, p, _. iFrame "∗ #". repeat iSplitR; auto.
-        iExists v. rewrite Hpwl. auto. }
-      assert (Hpub: related_sts_pub_world W (<s[l:=Temporary]s>W)).
-      { eapply (uninitialized_related_sts_pub_world l W); eauto. }
-      iDestruct (region_map_monotone _ _ _ _ Hpub with "Hmap_def") as "HMdef"; eauto.
-      iExists M,(<[l:=Temporary]>Mρ); iFrame.
-      assert (l ∈ dom (gset Addr) M) as Hin.
-      { rewrite -H1. apply elem_of_gmap_dom. eauto. }
-      repeat rewrite dom_insert_L.
-      repeat iSplit;[iPureIntro..|];[rewrite H1;set_solver|rewrite H2;set_solver|].
-      rewrite -delete_list_delete;auto. rewrite -delete_list_insert; auto. rewrite -HMeq.
-      rewrite delete_list_insert; auto. }
-    iFrame.
-  Qed.
-
-  Lemma region_close_next_uninit W ls l φ p w v `{forall Wv, Persistent (φ Wv)}:
-    l ∉ ls ->
-    sts_state_std l (Static {[l:=w]})
-    ∗ open_region_many (l::ls) W
-    ∗ l ↦ₐ[p] v
-    ∗ ⌜p ≠ O⌝
-    ∗ (if pwl p then future_pub_mono else future_priv_mono) φ v
-    ∗ ▷ φ (W,v) (* Maybe φ (<l[ l := Temporary, (Rpub, Rpriv) ]l> W, v) *)
-    ∗ rel l p φ
-    ∗ sts_full_world W
-    ==∗ open_region_many ls (<s[ l := Temporary ]s> W) ∗ sts_full_world (<s[ l := Temporary ]s> W).
-  Proof.
-    intros Hnotin. destruct (pwl p) eqn:Hpwl.
-    - iApply region_close_next_uninit_pwl; auto.
-    - iApply region_close_next_uninit_nwl; auto.
-  Qed.
-
-  Global Instance exi_uninit_eqdec l : Decision (∃ w : leibnizO Word, ρ' = Static {[l:=w]}).
-  Proof.
-    intros ρ; destruct ρ;[right|right|right|];[intros [? ?];done..|].
-    destruct (g !! l) eqn:Hsome;[|right];[|intros [? ?];simplify_map_eq].
-    destruct (decide (g = {[l:=w]}));[left|right];subst;eauto. intros [? ?]. simplify_map_eq.
-  Qed.
-
-  Lemma storeU_case (W : WORLD) (r : leibnizO Reg) (p p' : Perm) (g : Locality) (b e a : Addr) (w : Word) (ρ : region_type) (rdst : RegName) (offs rsrc : Z + RegName):
+   Lemma storeU_case (W : WORLD) (r : leibnizO Reg) (p p' : Perm) (g : Locality) (b e a : Addr) (w : Word) (ρ : region_type) (rdst : RegName) (offs rsrc : Z + RegName):
     ftlr_instr W r p p' g b e a w (StoreU rdst offs rsrc) ρ.
   Proof.
-    intros Hp Hsome i Hbae Hfp Hpwl Hregion [Hnotrevoked Hnotstatic] HO Hi.
+    intros Hp Hsome i Hbae Hfp Hpwl Hregion Hnotrevoked Hnotstatic Hnotmonostatic Hnotuninitialized HO Hi.
     iIntros "#IH #Hinv #Hreg #Hinva Hmono #Hw Hsts Hown".
     iIntros "Hr Hstate Ha HPC Hmap".
     rewrite delete_insert_delete.
     iDestruct ((big_sepM_delete _ _ PC) with "[HPC Hmap]") as "Hmap /=";
       [apply lookup_insert|rewrite delete_insert_delete;iFrame|]. simpl.
 
-    assert (Hsome': forall x, is_Some (<[PC:=inr (p, g, b, e, a)]> r !! x)).
-    { intros. destruct (reg_eq_dec x PC).
-      - subst x. rewrite lookup_insert; eauto.
-      - rewrite lookup_insert_ne; auto. }
-    destruct (Hsome' rdst) as [wdst Hrdst].
-    iDestruct (region_open_prepare with "Hr") as "Hr".
-    assert (Hwsrc: exists wsrc, word_of_argument (<[PC:=inr (p, g, b, e, a)]> r) rsrc = Some wsrc).
-    { destruct rsrc; eauto.
-      simpl; eapply Hsome'. }
-    destruct Hwsrc as [wsrc Hwsrc].
+    (* To read out PC's name later, and needed when calling wp_load *)
+    assert(∀ x : RegName, is_Some (<[PC:=inr (p, g, b, e, a)]> r !! x)) as Hsome'.
+    {
+      intros. destruct (decide (x = PC)).
+      rewrite e0 lookup_insert; unfold is_Some. by eexists.
+        by rewrite lookup_insert_ne.
+    }
 
-    iAssert (∃ (mem: gmap Addr (Perm * Word)),
-                ⌜let wx := <[PC:=inr (p, g, b, e, a)]> r !! rdst in
-                match wx with
-                | Some (inr (px, gx, bx, ex, ax)) =>
-                  if isU px && canStoreU px wsrc
-                  then let moffs := z_of_argument (<[PC:=inr (p, g, b, e, a)]> r) offs in
-                       match moffs with
-                       | Some zoffs =>
-                         let ma' := verify_access (StoreU_access bx ex ax zoffs) in
-                         match ma' with
-                         | Some a' =>
-                           let mpw := mem !! a' in
-                           match mpw with
-                           | Some (p'', w') => PermFlows (promote_perm px) p''
-                           | None => False
-                           end
-                         | None => True
-                         end
-                       | None => True
-                       end
-                  else True
-                | _ => True
-                end⌝ ∗
-                (▷ let wx := <[PC:=inr (p, g, b, e, a)]> r !! rdst in
-                match wx with
-                | Some (inr (px, gx, bx, ex, ax)) =>
-                  if isU px && canStoreU px wsrc
-                  then let moffs := z_of_argument (<[PC:=inr (p, g, b, e, a)]> r) offs in
-                       match moffs with
-                       | Some zoffs =>
-                         let ma' := verify_access (StoreU_access bx ex ax zoffs) in
-                         match ma' with
-                         | Some a' =>
-                           if addr_eq_dec ax a' then
-                             let mpw := mem !! a' in
-                             match mpw with
-                             | Some (p'', w') =>
-                               ⌜mem = if addr_eq_dec a a' then (<[a:=(p'',w)]> ∅) else <[a:=(p',w)]> (<[a':=(p'',w')]> ∅)⌝ ∗ sts_full_world W ∗ if addr_eq_dec a a' then open_region_many [a] W else region_open_resources_uninit W a' [a] p'' true
-                             | None => ⌜False⌝
-                             end
-                           else
-                             let mpw := mem !! a' in
-                             match mpw with
-                             | Some (p'', w') =>
-                               ⌜mem = if addr_eq_dec a a' then (<[a:=(p'',w)]> ∅) else <[a:=(p',w)]> (<[a':=(p'',w')]> ∅)⌝ ∗ sts_full_world W ∗ if addr_eq_dec a a' then open_region_many [a] W else region_open_resources W a' [a] p'' interpC w' true
-                             | None => ⌜False⌝
-                             end
-                         | None => True
-                         end
-                       | None => True
-                       end
-                  else True
-                | _ => True
-                end) ∗ ([∗ map] a↦pw ∈ mem, ∃ p w, ⌜pw = (p,w)⌝ ∗ a ↦ₐ[p] w) ∗ ⌜mem !! a = Some (p', w)⌝)%I
-        with "[Ha Hsts Hr]" as "H".
-    { rewrite Hrdst. destruct wdst; auto.
-      - iDestruct (memMap_resource_1 with "Ha") as "H".
-        iExists _; iFrame; auto. rewrite lookup_insert; auto.
-      - destruct_cap c. destruct (isU c && canStoreU c wsrc) eqn:HisU.
-        + destruct (z_of_argument (<[PC:=inr (p, g, b, e, a)]> r) offs) eqn:Hzof.
-          * destruct (verify_access (StoreU_access c2 c1 c0 z)) eqn:Hver.
-            -- apply andb_true_iff in HisU. destruct HisU as [HisU Hcan].
-               assert (Hdstne: rdst <> PC).
-               { red; intros; subst rdst.
-                 rewrite lookup_insert in Hrdst. inv Hrdst.
-                 destruct Hp as [-> | [-> | [-> ->] ] ]; simpl in HisU; inv HisU. }
-               iDestruct ("Hreg" $! rdst Hdstne) as "Hinvdst"; auto.
-               rewrite lookup_insert_ne in Hrdst; auto.
-               rewrite /RegLocate Hrdst.
-               eapply verify_access_spec in Hver.
-               destruct Hver as [HA [HB [HC HD] ] ].
-               destruct (addr_eq_dec c0 a0).
-               ++ (* Uninitialized stuff, HERE BE DRAGONS *)
-                  subst c0. destruct (addr_eq_dec a a0).
-                  ** subst a0. iDestruct (memMap_resource_1 with "Ha") as "H".
-                     iExists _; iFrame; auto.
-                     rewrite lookup_insert; auto.
-                     iSplitR; iFrame; auto.
-                     iDestruct (isU_limit_inv _ a with "Hinvdst") as "H"; auto.
-                     iDestruct "H" as (p'') "[% [Hun %]]".
-                     iAssert (⌜p' = p''⌝%I) as "%".
-                     { iDestruct (rel_agree with "[Hinva Hun]") as "[% A]".
-                       iSplit; [iExact "Hinva"| iExact "Hun"]. auto. }
-                     subst p'. iPureIntro. auto.
-                  ** iDestruct (isU_limit_inv _ a0 with "Hinvdst") as "H"; auto.
-                     iDestruct "H" as (p'') "[% [Hun %]]".
-                     destruct H0 as [ρ' [X [Y Z] ] ].
-                     iDestruct (region_open_next' with "[$Hsts $Hr]") as "HH"; eauto.
-                     { apply not_elem_of_cons. split; eauto.
-                       apply not_elem_of_nil. }
-                     iDestruct "HH" as (wa0) "(Hsts & Hstate & Hr & Ha0 & %)".
-                     iDestruct (memMap_resource_2ne with "[$Ha $Ha0]") as "H"; auto.
-                     iExists (<[a:=(p', w)]> (<[a0:=(_, wa0)]> ∅)).
-                     rewrite lookup_insert_ne; auto. rewrite lookup_insert.
+    (* Initializing the names for the values of Hsrc now, to instantiate the existentials in step 1 *)
+    assert (∃ p0 g0 b0 e0 a0 , read_reg_inr (<[PC:=inr (p, g, b, e, a)]> r) rdst p0 g0 b0 e0 a0) as [p0 [g0 [b0 [e0 [a0 HVdst] ] ] ] ].
+    {
+      specialize Hsome' with rdst as Hdst.
+      destruct Hdst as [wdst Hsomedst].
+      unfold read_reg_inr. destruct wdst. 2: destruct_cap c. all: repeat eexists.
+      right. by exists z. by left.
+    }
 
-                     iFrame. iSplitR; auto.
-                     iSplitL; [iSplitR;auto|].
-                     iExists _. iFrame. repeat iSplit;auto.
-                     iFrame "∗ #"; auto. rewrite lookup_insert; auto.
-               ++ iDestruct (isU_inv _ a0 with "Hinvdst") as "H"; auto.
-                  { split; solve_addr. }
-                  iDestruct "H" as (p'') "[% [X %]]".
-                  destruct (addr_eq_dec a a0).
-                  ** subst a0. iDestruct (memMap_resource_1 with "Ha") as "H".
-                     iExists _; iFrame; auto.
-                     rewrite lookup_insert; auto.
-                     iFrame. iSplitR; auto.
-                     iAssert (⌜p' = p''⌝)%I as %Hpeq.
-                     { rewrite /read_write_cond.
-                       iDestruct (rel_agree a p' p'' with "[$Hinva $X]") as "[$ A]". }
-                     subst p'. iPureIntro. auto.
-                  ** destruct H0 as [ρ' [X [Y Z ] ] ].
-                     iDestruct (region_open_next with "[$Hsts $Hr]") as "HH"; eauto.
-                     { intros [g' Hcontr]. subst. specialize (Z g'). contradiction. }
-                     { apply not_elem_of_cons. split; auto.
-                       apply not_elem_of_nil. }
-                     iDestruct "HH" as (w') "(Hsts & Hstate & Hr & Ha' & % & Hmono & HX)".
-                     iDestruct (memMap_resource_2ne with "[$Ha $Ha']") as "H"; auto.
-                     iExists (<[a:=(p', w)]> (<[a0:=(p'', w')]> ∅)).
-                     rewrite lookup_insert_ne; auto. rewrite lookup_insert.
-                     iFrame. iSplitR; auto.
-                     iSplitL; auto. iNext. iSplitR; auto.
-                     iExists ρ'. iFrame; auto. rewrite lookup_insert; auto.
-            -- iDestruct (memMap_resource_1 with "Ha") as "H".
-               iExists _; iFrame; auto. rewrite lookup_insert; auto.
-          * iDestruct (memMap_resource_1 with "Ha") as "H".
-            iExists _; iFrame; auto. rewrite lookup_insert; auto.
-        + iDestruct (memMap_resource_1 with "Ha") as "H".
-          iExists _; iFrame; auto. rewrite lookup_insert; auto. }
+     assert (∃ storev, word_of_argument (<[PC:=inr (p, g, b, e, a)]> r) rsrc = Some storev) as [storev Hwoa].
+    { destruct rsrc; cbn.
+      - by exists (inl z).
+      - specialize Hsome' with r0 as Hr0.
+        destruct Hr0 as [wsrc Hsomer0].
+        exists wsrc. by rewrite Hsomer0.
+    }
 
-    iDestruct "H" as (mem) "[% [A [B %]]]".
-    iApply (wp_storeU with "[Hmap B]"); eauto.
-    { simplify_map_eq; auto. }
+    (* Step 1: open the region, if necessary, and store all the resources obtained from the region in allow_load_res *)
+    iDestruct (create_store_res with "Hreg Hinva Hr Hsts") as "[HStoreRes Hsts]"; eauto.
+    { destruct Hp as [-> | [-> | [-> _] ] ];auto. }
+    { destruct Hp as [-> | [-> | [-> _] ] ];auto. }
+    (* Clear helper values; they exist in the existential now *)
+    clear HVdst p0 g0 b0 e0 a0 Hwoa storev.
+
+    (* Step2: derive the concrete map of memory we need, and any spatial predicates holding over it *)
+    iDestruct (store_res_implies_mem_map W  with "HStoreRes Ha") as (mem) "[HStoreMem HMemRes]".
+
+    (* Step 3:  derive the non-spatial conditions over the memory map*)
+    iDestruct (mem_map_implies_pure_conds _ _ _ _ _ _ _ _ _ _ offs with "HStoreMem") as %(HReadPC & HStoreAP); auto.
+
+    iApply (wp_storeU_alt with "[$Hmap $HMemRes]");[apply Hi|apply HO|eauto|auto..].
+    { by rewrite lookup_insert. }
     { rewrite /subseteq /map_subseteq /set_subseteq. intros rr _.
       apply elem_of_gmap_dom. rewrite lookup_insert_is_Some'; eauto. }
-    { rewrite Hrdst. rewrite Hrdst in H. destruct wdst; auto.
-      destruct_cap c. destruct (isU c && canStoreU c wsrc); auto.
-      destruct (z_of_argument (<[PC:=inr (p, g, b, e, a)]> r) offs); auto.
-      destruct (verify_access (StoreU_access c2 c1 c0 z)); auto.
-      destruct (mem !! a0); auto. destruct p0.
-      eapply PermFlows_trans; eauto. destruct c; econstructor. }
-    { iFrame. }
-    iNext. iIntros (r' mem' v) "[% [B C]]".
-    inv H1.
+    iNext. iIntros (regs' mem' retv). iDestruct 1 as (HSpec) "[Hmem Hmap]".
 
-    { rewrite Hrdst in H2. inv H2. rewrite Hwsrc in H3; inv H3.
-      rewrite Hrdst H4 H5 H6 H7 /=.
-      rewrite Hrdst H4 H5 H6 H7 /= in H.
-      iAssert (((fixpoint interp1) W) w0) as "#Hw0".
-      { rewrite /word_of_argument in Hwsrc.
-        destruct rsrc; inv Hwsrc.
-        - rewrite !fixpoint_interp1_eq /=; auto.
-        - destruct (reg_eq_dec PC r0).
-          + subst r0. rewrite lookup_insert in H2; inv H2.
-            rewrite (fixpoint_interp1_eq W (inr _)) /=.
-            iAssert (□ exec_cond W b e g p (fixpoint interp1))%I as "HinvPC".
-            { iModIntro. rewrite /exec_cond.
-              iIntros (a'' r'' W'' Hin) "#Hfuture".
-              iNext. rewrite /interp_expr /=.
-              iIntros "[[Hmap Hreg'] [Hfull [Hx [Hsts Hown]]]]".
-              iSplitR; eauto.
-              iApply ("IH" with "[Hmap] [Hreg'] [Hfull] [Hx] [Hsts] [Hown]"); iFrame "#"; eauto.
-              iModIntro. (* iExists p'. iSplitR; auto. *) simpl.
-              iDestruct "Hfuture" as %Hfuture.
-              iApply (big_sepL_mono with "Hinv"); intros; simpl.
-              iIntros "H". iDestruct "H" as (? ?) "[HA %]". iExists _; iSplit;eauto. iFrame. iPureIntro.
-              destruct (pwl p) eqn:Hpwlp.
-              - eapply region_state_pwl_monotone; eauto.
-                destruct Hp as [-> | [-> | [-> ->] ] ]; simpl in Hpwlp; try congruence.
-              - destruct g; [eapply region_state_nwl_monotone_nl; eauto| eapply region_state_nwl_monotone; eauto].
-            }
-            destruct Hp as [-> | [-> | [-> ->] ] ]; iFrame "#"; auto.
-          + rewrite lookup_insert_ne in H2; auto.
-            iDestruct ("Hreg" $! r0 ltac:(auto)) as "HX"; auto.
-            rewrite /RegLocate H2. auto. }
-      assert (Hnedst: rdst <> PC).
-      { red; intro; subst rdst. rewrite lookup_insert in Hrdst.
-        inv Hrdst. destruct Hp as [-> | [-> | [-> ->] ] ]; simpl in H4; inv H4. }
-      iDestruct ("Hreg" $! rdst Hnedst) as "Hwdst".
-      rewrite lookup_insert_ne in Hrdst; auto.
-      rewrite /RegLocate Hrdst.
-      iAssert (|==> ∃ W', region W' ∗ ⌜related_sts_pub_world W W'⌝ ∗ sts_full_world W' ∗ if addr_eq_dec a0 a' then match (a0 + 1)%a with | Some a'' => ((fixpoint interp1) W') (inr (p0, g0, b0, e0, a'')) | None => True end else True)%I with "[A B Hmono Hstate]" as ">HW".
-      { destruct (addr_eq_dec a0 a').
-        - subst a0. destruct (a' + 1)%a as [a''|] eqn:Hap1; try tauto.
-          destruct (mem !! a') as [(p'', w'')|]; auto.
-          iDestruct "A" as "[% [Hsts A]]".
-          destruct (addr_eq_dec a a').
-          + iModIntro; subst a'; subst mem.
-            iDestruct (region_open_prepare with "A") as "A".
-            rewrite insert_insert.
-            iDestruct (memMap_resource_1 with "B") as "B".
-            inv H8. rewrite lookup_insert in H0; inv H0.
-            iDestruct (region_close _ _ (λ Wv : (WORLD * Word), interp Wv.1 Wv.2)
-                         with "[$A $B $Hstate Hmono]") as "B"; eauto.
-            { destruct ρ; auto; congruence. }
-            { iFrame "#". iSplitR; auto.
-              destruct (decide (ρ = Temporary ∧ pwl p' = true)).
-              - rewrite /future_pub_mono /=. iModIntro.
-                iIntros (W1 W2) "% #A".
-                iApply interp_monotone; auto.
-              - rewrite /future_priv_mono /=. iModIntro.
-                iIntros (W1 W2) "% #A". iApply (interp_monotone_nl with "[] [] A"); auto.
-                destruct w0; auto.
-                eapply not_and_r in n. destruct_cap c.
-                simpl. destruct c3; auto. simpl in H5.
-                destruct (pwlU p0) eqn:HwplU; intros; try congruence.
-                destruct n.
-                * iAssert (⌜g0 = Local⌝)%I as %->.
-                  { rewrite (fixpoint_interp1_eq W (inr (p0, _, _, _, _))).
-                    destruct p0; simpl in HwplU; try congruence; destruct g0; simpl; auto. }
-                  rewrite (fixpoint_interp1_eq W (inr (p0, _, _, _, _))).
-                  iAssert (⌜region_state_U_pwl W a⌝)%I as %Hρ.
-                  { destruct p0; simpl in H,H4,H5,H6,HwplU; try congruence.
-                    - simpl. iDestruct "Hwdst" as "[YA YB]".
-                      destruct (proj1 (verify_access_spec _ _) H7) as (A & B & C & D).
-                      iDestruct (extract_from_region_inv with "YB") as (pp ?) "[E %]"; auto.
-                      split; try solve_addr.
-                    - simpl. iDestruct "Hwdst" as "[YA YC]".
-                      destruct (proj1 (verify_access_spec _ _) H7) as (A & B & C & D).
-                      iDestruct (extract_from_region_inv with "YC") as (pp ?) "[E %]"; auto.
-                      split; try solve_addr. }
-                  destruct Hρ as [Hρ | Hρ]; rewrite Hregion in Hρ; inversion Hρ; try subst ρ; congruence.
-                * assert (HpwlU2: pwlU p' = true).
-                  { destruct p0; simpl in H6; simpl in HwplU; try congruence; destruct p'; rewrite /PermFlows in H; inv H; simpl in H0; try congruence; reflexivity. }
-                  destruct Hp as [-> | [-> | [-> ->] ] ]; destruct p'; simpl in HpwlU2; simpl in H0; try congruence; inv Hfp. }
-            iExists W. iFrame. iSplitR.
-            * iPureIntro.
-              rewrite /related_sts_pub_world; eapply related_sts_pub_refl_world.
-            * rewrite !(fixpoint_interp1_eq W (inr (p0,_,_,_,_))) !interp1_eq.
-              destruct (perm_eq_dec p0 O); [subst p0; simpl in H4; congruence|].
-              destruct (perm_eq_dec p0 E); [subst p0; simpl in H4; congruence|].
-              iDestruct "Hwdst" as "[A1 [% A4]]".
-              rewrite H4. iFrame "%".
-              destruct g0; simpl; iFrame "#". eapply verify_access_spec in H7.
-              destruct H7 as [A1 [A2 [A3 A4] ] ].
-              replace (addr_reg.max b0 a) with a by solve_addr.
-              replace (addr_reg.min a e0) with a by solve_addr.
-              replace (addr_reg.min a'' e0) with a'' by solve_addr.
-              iSplit.
-              { rewrite (isWithin_region_addrs_decomposition a a'' b0 a''); [|solve_addr].
-                iApply big_sepL_app. iFrame "#".
-                iApply big_sepL_app.
-                replace (region_addrs a'' a'') with (@nil Addr) by (rewrite /region_addrs region_size_0 /=; auto; solve_addr).
-                iSplitL.
-                - replace (region_addrs a a'') with (a::nil).
-                  + iApply big_sepL_cons. iSplitL; [|iApply big_sepL_nil; auto].
-                    iDestruct (extract_from_region_inv a e0 a with "A4") as (pp ?) "[X1 %]"; [solve_addr|].
-                    iExists pp. iSplit;auto. iSplitL; auto.
-                    iPureIntro; auto.
-                    destruct (pwlU p0) eqn:Hp0.
-                    { rewrite /region_state_U_pwl in H2. destruct H2; auto.
-                      destruct H2.
-                      eelim Hnotstatic. congruence. }
-                    { rewrite /region_state_U_pwl in H2. destruct H2; auto.
-                      destruct H2; auto. destruct H2. eelim Hnotstatic. congruence. }
-                  + rewrite /region_addrs /region_size /=.
-                    replace (a'' - a)%Z with 1%Z by solve_addr.
-                    simpl. auto.
-                - iApply big_sepL_nil; auto. }
-              { replace (addr_reg.max b0 a'') with a'' by solve_addr.
-                iApply (big_sepL_submseteq with "A4").
-                rewrite (region_addrs_decomposition a a e0); [|solve_addr].
-                replace ^(a + 1)%a with a'' by solve_addr.
-                eapply submseteq_inserts_l.
-                eapply submseteq_cons. auto. }
-          + subst mem. iDestruct "A" as (ρ') "[A1 [ [% %] [A2 [% #A3]]]]".
-            iDestruct (sts_full_state_std with "[$Hsts] [$A1]") as "%".
-            (* destruct (region_type_EqDecision ρ' Uninitialized). *)
-            destruct (decide (exists w, ρ' = Static {[a':=w]})).
-            * destruct e1 as [? e1]. subst ρ'. rewrite -(insert_delete _ a' (p'0, w0)).
-              rewrite delete_insert_ne; auto. rewrite delete_insert; auto.
-              iDestruct (memMap_resource_2ne with "B") as "[B1 B2]"; auto. inv H8.
-              iDestruct (region_close_next_uninit with "[$A1 $A2 $B1 $A3 $Hw0 $Hsts]") as "HX".
-              { eapply not_elem_of_cons; split; auto.
-                eapply not_elem_of_nil. }
-              { iSplitR; auto. simpl. destruct (pwl p'0) eqn:Hpwl'.
-                - rewrite /future_pub_mono /=. iModIntro.
-                  iIntros (W1 W2) "% #A".
-                  iApply interp_monotone; auto.
-                - rewrite /future_priv_mono /=. iModIntro.
-                  iIntros (W1 W2) "% #A". iApply interp_monotone_nl; auto.
-                  destruct w0; auto.
-                  destruct_cap c. simpl. destruct c3; auto.
-                  simpl in H5. destruct (pwlU p0) eqn:HpwlU; try congruence.
-                  exfalso. destruct p0; simpl in H,H4,HpwlU; try congruence;
-                  destruct p'0; simpl in *; inv H; congruence. }
-              iDestruct "HX" as ">[Hregion Hfull]".
-              iDestruct (region_open_prepare with "Hregion") as "Hregion".
-              assert (related_sts_pub_world W (<s[a':=Temporary]s>W)).
-              { eapply (uninitialized_related_sts_pub_world); eauto. }
-              iDestruct (region_close with "[$Hregion $B2 $Hstate $Hmono]") as "HH"; eauto.
-              { destruct ρ;auto; congruence. }
-              { iSplitR; auto. iFrame "∗ #". iNext.
-                iApply interp_monotone; auto. }
-              iModIntro. iExists _. iFrame "∗ %".
-              iDestruct (interp_monotone with "[] [$Hwdst]") as "#Hwdst'"; [iPureIntro; eauto|].
-              rewrite !(fixpoint_interp1_eq (<s[a':=_]s> W)) !interp1_eq.
-              destruct (perm_eq_dec p0 O); [subst p0; simpl in H8; discriminate|].
-              destruct (perm_eq_dec p0 E); [subst p0; simpl in H8; discriminate|].
-              iDestruct "Hwdst'" as "[A1 [% A4]]".
-              rewrite H4. iFrame "%".
-              destruct g0; simpl; iFrame "#". eapply verify_access_spec in H7.
-              destruct H7 as [A1 [A2 [A3 A4] ] ].
-              replace (addr_reg.max b0 a') with a' by solve_addr.
-              replace (addr_reg.min a' e0) with a' by solve_addr.
-              replace (addr_reg.min a'' e0) with a'' by solve_addr.
-              iSplit.
-              { rewrite (isWithin_region_addrs_decomposition a' a'' b0 a''); [|solve_addr].
-                iApply big_sepL_app. iFrame "#".
-                iApply big_sepL_app.
-                replace (region_addrs a'' a'') with (@nil Addr) by (rewrite /region_addrs region_size_0 /=; auto; solve_addr).
-                iSplitL.
-                - replace (region_addrs a' a'') with (a'::nil).
-                  + iApply big_sepL_cons. iSplitL; [|iApply big_sepL_nil; auto].
-                    iDestruct (extract_from_region_inv a' e0 a' with "A4") as (pp ?) "[X1 %]"; [solve_addr|].
-                    iExists pp; iSplit;auto. iSplitL; auto.
-                    iPureIntro; auto.
-                    destruct (pwlU p0) eqn:Hp0; auto.
-                    { rewrite /region_state_pwl /std_update /std /=.
-                      rewrite lookup_insert. reflexivity. }
-                    { rewrite /region_state_pwl /std_update /std /=.
-                      rewrite lookup_insert. auto. }
-                  + rewrite /region_addrs /region_size /=.
-                    replace (a'' - a')%Z with 1%Z by solve_addr.
-                    simpl. auto.
-                - iApply big_sepL_nil; auto. }
-              { replace (addr_reg.max b0 a'') with a'' by solve_addr.
-                iApply (big_sepL_submseteq with "A4").
-                rewrite (region_addrs_decomposition a' a' e0); [|solve_addr].
-                replace ^(a' + 1)%a with a'' by solve_addr.
-                eapply submseteq_inserts_l.
-                eapply submseteq_cons. auto. }
-            * rewrite -(insert_delete _ a' (p'0, w0)).
-              rewrite delete_insert_ne; auto. rewrite delete_insert; auto.
-              iDestruct (memMap_resource_2ne with "B") as "[B1 B2]"; auto. inv H8.
-              iDestruct (region_close_next with "[$A1 $A2 $B1 $A3 $Hw0]") as "HX"; auto.
-              { intros [g' Hcontr]. specialize (H2 g'). apply H2 in Hcontr as Hcontr'. destruct Hcontr'. subst g'.
-                simplify_map_eq.
-                assert (∃ w : leibnizO Word, Static {[a' := x]} = Static {[a' := w]});eauto. }
-              { eapply not_elem_of_cons; split; auto.
-                eapply not_elem_of_nil. }
-              { iSplitR; auto. rewrite /monotonicity_guarantees_region.
-                destruct ρ'; auto.
-                - destruct (pwl p'0) eqn:Hpwl'.
-                  + rewrite /future_pub_mono /=. iModIntro.
-                    iIntros (W1 W2) "% #A".
-                    iApply interp_monotone; auto.
-                  + rewrite /future_priv_mono /=. iModIntro.
-                    iIntros (W1 W2) "% #A". iApply interp_monotone_nl; auto.
-                    destruct w0; auto.
-                    destruct_cap c. simpl. destruct c3; auto.
-                    simpl in H7. destruct (pwlU p0) eqn:HpwlU; try congruence; exfalso;
-                    destruct p0; simpl in H,H4,HpwlU; try congruence;
-                      destruct p'0; simpl in *; inv H; congruence.
-                - simpl. rewrite /future_priv_mono /=. iModIntro.
-                  iIntros (W1 W2) "% #A". iApply interp_monotone_nl; auto.
-                  destruct w0; auto. destruct_cap c. simpl. destruct c3; auto.
-                  simpl in H5. destruct p0; simpl in H4, H5; try (inv H4; inv H5; fail).
-                  + rewrite (fixpoint_interp1_eq W (inr (URWL,_,_,_,_))) /=.
-                    destruct g0; auto. iDestruct "Hwdst" as "[Y1 Y2]".
-                    iDestruct (extract_from_region_inv _ _ a' with "Y2") as (pp ?) "[Y3 %]".
-                    { eapply verify_access_spec in H7.
-                      destruct H7 as [X1 [X2 [X3 X4] ] ].
-                      solve_addr. }
-                    destruct H11;[|destruct H11]; rewrite H11 in H9; discriminate.
-                  + rewrite (fixpoint_interp1_eq W (inr (URWLX,_,_,_,_))) /=.
-                    destruct g0; auto. iDestruct "Hwdst" as "[Y1 Y3]".
-                    iDestruct (extract_from_region_inv _ _ a' with "Y3") as (pp ?) "[Y4 %]".
-                    { eapply verify_access_spec in H7.
-                      destruct H7 as [X1 [X2 [X3 X4] ] ].
-                      solve_addr. }
-                    destruct H11;[|destruct H11]; rewrite H11 in H9; discriminate. }
-              iDestruct (region_open_prepare with "HX") as "Hregion".
-              iDestruct (region_close with "[$Hregion $B2 $Hstate $Hmono]") as "HH"; eauto.
-              { destruct ρ;auto;congruence. }
-              iModIntro. iExists _. iFrame "∗ %". iSplit.
-              { iPureIntro. rewrite /related_sts_pub_world; eapply related_sts_pub_refl_world. }
-              { rewrite !(fixpoint_interp1_eq W (inr (p0,_,_,_,_))) !interp1_eq.
-                destruct (perm_eq_dec p0 O); [subst p0; simpl in *; congruence|].
-                destruct (perm_eq_dec p0 E); [subst p0; simpl in *; congruence|].
-                iDestruct "Hwdst" as "[A1 [% A4]]".
-                rewrite H4. iFrame "%".
-                destruct g0; simpl; iFrame "#". eapply verify_access_spec in H7.
-                destruct H7 as [A1 [A2 [A3 A4] ] ].
-                replace (addr_reg.max b0 a') with a' by solve_addr.
-                replace (addr_reg.min a' e0) with a' by solve_addr.
-                replace (addr_reg.min a'' e0) with a'' by solve_addr.
-                iSplit.
-                { rewrite (isWithin_region_addrs_decomposition a' a'' b0 a''); [|solve_addr].
-                  iApply big_sepL_app. iFrame "#".
-                  iApply big_sepL_app.
-                  replace (region_addrs a'' a'') with (@nil Addr) by (rewrite /region_addrs region_size_0 /=; auto; solve_addr).
-                  iSplitL.
-                  - replace (region_addrs a' a'') with (a'::nil).
-                    + iApply big_sepL_cons. iSplitL; [|iApply big_sepL_nil; auto].
-                      iDestruct (extract_from_region_inv a' e0 a' with "A4") as (pp Hflowspp) "[X1 %]"; [solve_addr|].
-                      iExists pp; iSplit;auto. iSplitL; auto.
-                      iPureIntro;auto.
-                      destruct (pwlU p0) eqn:Hp0; auto.
-                      { destruct H7; auto. elim n0.
-                        rewrite H9 in H7; inv H7. exists x. inversion H11. eauto. }
-                      { destruct H7; auto. destruct H7; auto. elim n0. destruct H7.
-                        rewrite H7 in H9; inv H9. eauto. }
-                    + rewrite /region_addrs /region_size /=.
-                      replace (a'' - a')%Z with 1%Z by solve_addr.
-                      simpl. auto.
-                  - iApply big_sepL_nil; auto. }
-                { replace (addr_reg.max b0 a'') with a'' by solve_addr.
-                  iApply (big_sepL_submseteq with "A4").
-                  rewrite (region_addrs_decomposition a' a' e0); [|solve_addr].
-                  replace ^(a' + 1)%a with a'' by solve_addr.
-                  eapply submseteq_inserts_l.
-                  eapply submseteq_cons. auto. } }
-        - iModIntro. destruct (mem !! a') as [(p'', w'')|]; auto.
-          iDestruct "A" as "[% [Hsts A]]".
-          destruct (addr_eq_dec a a').
-          + subst a'. subst mem.
-            iDestruct (region_open_prepare with "A") as "A".
-            rewrite insert_insert.
-            iDestruct (memMap_resource_1 with "B") as "B".
-            rewrite lookup_insert in H0.
-            inversion H8; inversion H0. subst p'' w'' p'0.
-            iDestruct (region_close _ _ (λ Wv : WORLD * Word, interp Wv.1 Wv.2) with "[$A $B $Hstate Hmono]") as "B"; eauto.
-            { destruct ρ;auto;congruence. }
-            { iSplitR;auto. iFrame "#". simpl.
-              destruct (decide (ρ = Temporary ∧ pwl p' = true)).
-              - rewrite /future_pub_mono /=. iModIntro.
-                 iIntros (W1 W2) "% #A".
-                 iApply interp_monotone; auto.
-              - rewrite /future_priv_mono /=. iModIntro.
-                 iIntros (W1 W2) "% #A". iApply interp_monotone_nl; auto.
-                 destruct w0; auto.
-                 eapply not_and_r in n0. destruct_cap c.
-                 simpl. destruct c3; auto. simpl in H5.
-                 destruct (pwlU p0) eqn:HwplU; intros; try congruence.
-                 destruct n0.
-                 * iAssert (⌜g0 = Local⌝)%I as %->.
-                    { rewrite (fixpoint_interp1_eq W (inr (p0, _, _, _, _))).
-                      destruct p0; simpl in HwplU; try congruence; destruct g0; simpl; auto. }
-                    rewrite (fixpoint_interp1_eq W (inr (p0, _, _, _, _))).
-                    iAssert (⌜region_state_U_pwl W a⌝)%I as %Hρ.
-                    { destruct p0; simpl in H4; simpl in HwplU; try congruence.
-                      - simpl. iDestruct "Hwdst" as "[YA YB]".
-                        destruct (proj1 (verify_access_spec _ _) H7) as (A & B & C & D).
-                        iDestruct (extract_from_region_inv _ _ a with "YA") as (pp ?) "[E %]"; auto.
-                        split; try solve_addr. rewrite /addr_reg.min; destruct (Addr_le_dec a0 e0); solve_addr.
-                      - simpl. iDestruct "Hwdst" as "[YA YB]".
-                        destruct (proj1 (verify_access_spec _ _) H7) as (A & B & C & D).
-                        iDestruct (extract_from_region_inv _ _ a with "YA") as (pp ?) "[E %]"; auto.
-                        split; try solve_addr. rewrite /addr_reg.min; destruct (Addr_le_dec a0 e0); solve_addr. }
-                    destruct Hρ as [Hρ | Hρ]; rewrite Hregion in Hρ; inversion Hρ; try subst ρ; congruence.
-                  * assert (HpwlU2: pwlU p' = true).
-                    { destruct p0; simpl in H5; simpl in HwplU; try congruence; destruct p'; rewrite /PermFlows in H; inv H; simpl in H0; try congruence; reflexivity. }
-                    exfalso. destruct Hp as [-> | [-> | [-> ->] ] ]; destruct p'; simpl in HpwlU2; simpl in *; try congruence; inv Hfp. }
+    destruct HSpec as [* ? ? ? ? ? -> Hincr|].
+    { destruct (addr_eq_dec a0 a').
+      - subst. destruct (a' + 1)%a eqn:Hincr';inversion Hincr. 
+        apply incrementPC_Some_inv in Hincr.
 
-            iExists W. iFrame. iPureIntro. apply related_sts_pub_refl_world.
-          + subst mem. rewrite insert_commute; auto.
-            rewrite insert_insert.
-            iDestruct (memMap_resource_2ne with "B") as "[B C]"; auto.
-            rewrite /region_open_resources.
-            iDestruct "A" as (ρ') "[A1 [ [% %] [A2 [% [[A3 #Hw'] #A4]]]]]". inv H8.
-            iDestruct (sts_full_state_std with "[$Hsts] [$A1]") as "%".
-            iDestruct (region_close_next with "[$A1 $A2 A3 $A4 $C]") as "A"; auto.
-            { intros [g' Hcontr]. specialize (H2 g'). congruence. }
-            { eapply not_elem_of_cons; split; auto. eapply not_elem_of_nil. }
-            { iSplitR; auto. simpl. iSplit; auto.
-              rewrite !switch_monotonicity_formulation; auto.
-              rewrite /monotonicity_guarantees_decide.
-              destruct (decide (ρ' = Temporary ∧ pwl p'0 = true)).
-              + rewrite /future_pub_mono /=. iModIntro.
-                iIntros (W1 W2) "% #A".
-                iApply interp_monotone; auto.
-              + rewrite /future_priv_mono /=. iModIntro.
-                iIntros (W1 W2) "% #A". iApply interp_monotone_nl; auto.
-                destruct w0; auto.
-                eapply not_and_r in n1. destruct_cap c.
-                simpl. destruct c3; auto. simpl in H4,H5.
-                destruct (pwlU p0) eqn:HwplU; intros; try congruence.
-                destruct n1.
-                * iAssert (⌜g0 = Local⌝)%I as %->.
-                  { rewrite (fixpoint_interp1_eq W (inr (p0, _, _, _, _))).
-                    destruct p0; simpl in HwplU; try congruence; destruct g0; simpl; auto. }
-                  rewrite (fixpoint_interp1_eq W (inr (p0, _, _, _, _))).
-                  iAssert (⌜region_state_U_pwl W a'⌝)%I as %Hρ.
-                  { destruct p0; simpl in H4; simpl in HwplU; try congruence.
-                    - simpl. iDestruct "Hwdst" as "[YA YB]".
-                      destruct (proj1 (verify_access_spec _ _) H7) as (A & B & C & D).
-                      iDestruct (extract_from_region_inv b0 _ a' with "YA") as (pp ?) "[E %]"; auto.
-                      split; try solve_addr. iPureIntro. left; auto.
-                    - simpl. iDestruct "Hwdst" as "[YA YC]".
-                      destruct (proj1 (verify_access_spec _ _) H7) as (A & B & C & D).
-                      iDestruct (extract_from_region_inv b0 _ a' with "YA") as (pp ?) "[E %]"; auto.
-                      split; try solve_addr. iPureIntro. left; auto. }
-                  destruct Hρ as [Hρ | Hρ]; rewrite H8 in Hρ; inversion Hρ; try subst ρ'; congruence.
-                * assert (HpwlU2: pwlU p'0 = true).
-                  { destruct p0; simpl in H5; simpl in HwplU; try congruence; destruct p'0; rewrite /PermFlows in H; inv H; simpl in H0; try congruence; reflexivity. }
-                  exfalso. destruct p0; destruct p'0; simpl in H5, HwplU, HpwlU2, H10; try congruence; inv H; auto. }
-            iDestruct (region_open_prepare with "A") as "A".
-            iDestruct (region_close with "[$A $B $Hmono $Hstate]") as "B"; auto.
-            { destruct ρ;auto;congruence. }
-            iExists W. iFrame. iPureIntro. apply related_sts_pub_refl_world. }
-      iDestruct "HW" as (W') "[Hregion [% [Hfull HX]]]".
-      iDestruct ("IH" $! W' r' with "[] [HX] [C] [$Hregion] [$Hfull] [$Hown] [] []") as "H"; auto.
-      { iPureIntro. simpl; intros.
-        destruct (addr_eq_dec a0 a').
-        - subst a0. destruct (a' + 1)%a as [a''|] eqn:Ha'; try tauto.
-          eapply incrementPC_Some_inv in H10.
-          destruct H10 as (?&?&?&?&?&?&?&?&?).
-          subst r'. destruct (reg_eq_dec PC x).
-          * subst x; rewrite lookup_insert; eauto.
-          * rewrite lookup_insert_ne; auto.
-            destruct (reg_eq_dec rdst x).
-            { subst x. rewrite lookup_insert; eauto. }
-            { rewrite !lookup_insert_ne; auto. }
-        - eapply incrementPC_Some_inv in H10.
-          destruct H10 as (?&?&?&?&?&?&?&?&?).
-          subst r'. destruct (reg_eq_dec PC x).
-          + subst x; rewrite lookup_insert; eauto.
-          + rewrite !lookup_insert_ne; auto. }
-      { iIntros (x) "%".
-        destruct (addr_eq_dec a0 a').
-        - subst a0. destruct (a' + 1)%a as [a''|] eqn:Ha'; try tauto.
-          eapply incrementPC_Some_inv in H10.
-          destruct H10 as (?&?&?&?&?&?&?&?&?).
-          subst r'. rewrite lookup_insert_ne; auto.
-          destruct (reg_eq_dec rdst x).
-          * subst x. rewrite lookup_insert. auto.
-          * rewrite !lookup_insert_ne; auto.
-            iApply interp_monotone; auto.
-            iApply "Hreg"; auto.
-        - eapply incrementPC_Some_inv in H10.
-          destruct H10 as (?&?&?&?&?&?&?&?&?).
-          subst r'. rewrite !lookup_insert_ne; auto.
-          iApply interp_monotone; auto.
-          iApply "Hreg"; auto. }
-      { instantiate (3 := b).
-        instantiate (2 := e).
-        instantiate (1 := match (a + 1)%a with Some a' => a' | None => a end).
-        destruct (addr_eq_dec a0 a').
-        - subst a0. destruct (a' + 1)%a as [a''|] eqn:Ha'; try tauto.
-          eapply incrementPC_Some_inv in H10.
-          destruct H10 as (?&?&?&?&?&?&?&?&?).
-          subst r'. rewrite insert_insert.
-          simplify_map_eq. auto.
-        - eapply incrementPC_Some_inv in H10.
-          destruct H10 as (?&?&?&?&?&?&?&?&?).
-          subst r'. rewrite insert_insert.
-          simplify_map_eq. rewrite insert_insert;auto. }
-      { iModIntro. (* iExists p'; iSplitR; auto. *)
-        iApply (big_sepL_mono with "Hinv"); auto.
-        intros. simpl. iIntros "Hw". iDestruct "Hw" as (pp ?) "Hw".
-        iExists pp; iSplit;auto.
-        iDestruct "Hw" as "[$ %]".
-        destruct (pwl p);iPureIntro.
-        + eapply region_state_pwl_monotone; eauto.
-        + eapply region_state_nwl_monotone; eauto.
-      }
-      iApply wp_pure_step_later; auto. iNext.
-      iApply (wp_mono with "H"). simpl.
-      iIntros (v) "H %". iDestruct ("H" $! a1) as (rx Wx) "[A [B [% [C [D E]]]]]".
-      iExists rx, Wx; iFrame.
-      iPureIntro. eapply related_sts_priv_trans_world; eauto.
-      eapply related_sts_pub_priv_world; auto. }
+        destruct Hincr as (?&?&?&?&?&?&?&?&?).
+        iApply wp_pure_step_later; auto. iNext.
+
+        (* From this, derive value relation for the current PC*)
+        iDestruct (execcPC_implies_interp _ _ _ _ _ a  with "Hinv") as "HVPC"; eauto.
+
+        iDestruct (switch_monotonicity_formulation with "Hmono") as "Hmono"; [eauto..|].
+
+        (* Step 4: return all the resources we had in order to close the second location in the region, in the cases where we need to *)
+        iMod (mem_map_recover_res with "HStoreMem Hreg HVPC Hw Hmono Hmem Hsts") as (w') "(Hr & Hsts & Ha & #HSVInterp & Hmono & %)";eauto.
+        { destruct Hp as [-> | [-> | [-> _] ] ];auto. }
+
+        iDestruct (switch_monotonicity_formulation with "Hmono") as "Hmono"; auto.
+
+        iDestruct (region_close with "[$Hstate $Hr $Ha $Hmono]") as "Hr"; eauto.
+        { destruct ρ;auto;[|specialize (Hnotstatic g1)|specialize (Hnotmonostatic g1)|specialize (Hnotuninitialized w1)];try contradiction. }
+        simplify_map_eq.
+
+        iApply wp_wand_r.
+        iSplitL. iApply ("IH" $! (new_worldU W a' p g b e a r offs) with "[%] [] [$Hmap] [$Hr] [$Hsts] [$Hown]"); auto.
+        { cbn. intros x'. destruct (decide (rdst = x'));simplify_map_eq;eauto. }
+        { iIntros (r1 Hne). destruct (decide (rdst = r1)).
+          { subst. rewrite /RegLocate. assert (Hval:=H2).
+            destruct H2 as [Hdst H2]. simplify_map_eq.
+            iSpecialize ("Hreg" $! r1 Hne). rewrite Hdst.
+            iApply (interp_initialize_limit with "Hreg");eauto. }
+          { rewrite /RegLocate. simplify_map_eq. iSpecialize ("Hreg" $! r1 Hne).
+            destruct (r !! r1) eqn:Hsomer;rewrite Hsomer.
+            iApply (interp_monotone with "[] Hreg"). auto.
+            rewrite !fixpoint_interp1_eq. done. 
+          }
+        }
+        { iPureIntro. destruct (decide (rdst = PC));subst;[|simplify_map_eq;auto].
+          unfold reg_allows_storeU in H2. 
+          rewrite /incrementPC in H5. simplify_map_eq. destruct H2 as [H2 _]. inversion H2;subst;auto. }
+        { destruct (decide (rdst = PC));subst;simplify_map_eq;auto.
+          - unfold reg_allows_storeU in H2. 
+            rewrite /incrementPC in H5. simplify_map_eq.
+            destruct H2 as [H2 _]. inversion H2;subst;auto.
+            iDestruct (interp_monotone with "[] HVPC") as "HVPC'";[iPureIntro;apply H8|].
+            iClear "Hw HSVInterp HVPC".
+            rewrite fixpoint_interp1_eq /=.
+            destruct Hp as [-> | [-> | [-> _] ] ]; try iFrame "HVPC'". destruct x0; try done; iFrame "HVPC'". 
+          - iDestruct (interp_monotone with "[] HVPC") as "HVPC'";[iPureIntro;apply H8|].
+            iClear "Hw HSVInterp HVPC".
+            rewrite fixpoint_interp1_eq /=.
+            destruct Hp as [-> | [-> | [-> _] ] ]; try iFrame "HVPC'". destruct x0; try done; iFrame "HVPC'". 
+        }
+        iIntros (v) "Hv". iIntros (Hhalted).
+        iDestruct ("Hv" $! Hhalted) as (r0 W') "(Hfull & Hregs & % & Hown & sts & Hr)".
+        iExists _,_. iFrame. iPureIntro. eapply related_sts_pub_priv_trans_world;eauto.
+      - apply incrementPC_Some_inv in Hincr.
+
+        destruct Hincr as (?&?&?&?&?&?&?&?&?).
+        iApply wp_pure_step_later; auto. iNext.
+
+        (* From this, derive value relation for the current PC*)
+        iDestruct (execcPC_implies_interp _ _ _ _ _ a  with "Hinv") as "HVPC"; eauto.
+
+        iDestruct (switch_monotonicity_formulation with "Hmono") as "Hmono"; [eauto..|].
+
+        (* Step 4: return all the resources we had in order to close the second location in the region, in the cases where we need to *)
+        iMod (mem_map_recover_res with "HStoreMem Hreg HVPC Hw Hmono Hmem Hsts") as (w') "(Hr & Hsts & Ha & #HSVInterp & Hmono & %)";eauto.
+        { destruct Hp as [-> | [-> | [-> _] ] ];auto. }
+
+        iDestruct (switch_monotonicity_formulation with "Hmono") as "Hmono"; auto.
+
+        iDestruct (region_close with "[$Hstate $Hr $Ha $Hmono]") as "Hr"; eauto.
+        { destruct ρ;auto;[|specialize (Hnotstatic g1)|specialize (Hnotmonostatic g1)|specialize (Hnotuninitialized w1)];try contradiction. }
+        simplify_map_eq.
+        
+        iApply wp_wand_r.
+        iSplitL. iApply ("IH" $! (new_worldU W a0 x x0 x1 x2 x3 r offs) with "[%] [] [$Hmap] [$Hr] [$Hsts] [$Hown]"); auto.
+        { iIntros (r1 Hne). destruct (decide (rdst = r1)).
+          { subst. rewrite /RegLocate. assert (Hval:=H2).
+            destruct H2 as [Hdst H2]. simplify_map_eq.
+            iSpecialize ("Hreg" $! r1 Hne). rewrite Hdst.
+            iApply (interp_monotone with "[] Hreg"). auto. }
+          { rewrite /RegLocate. simplify_map_eq. iSpecialize ("Hreg" $! r1 Hne).
+            destruct (r !! r1) eqn:Hsomer;rewrite Hsomer.
+            iApply (interp_monotone with "[] Hreg"). auto.
+            rewrite !fixpoint_interp1_eq. done. 
+          }
+        }
+        { destruct (decide (rdst = PC));subst;simplify_map_eq;auto.
+          - unfold reg_allows_storeU in H2. 
+            rewrite /incrementPC in H5. simplify_map_eq.
+            destruct H2 as [H2 _]. inversion H2;subst;auto.
+            iDestruct (interp_monotone with "[] HVPC") as "HVPC'";[iPureIntro;apply H7|].
+            iClear "Hw HSVInterp HVPC".
+            rewrite fixpoint_interp1_eq /=.
+            destruct Hp as [-> | [-> | [-> _] ] ]; try iFrame "HVPC'". destruct g0; try done; iFrame "HVPC'". 
+          - iDestruct (interp_monotone with "[] HVPC") as "HVPC'";[iPureIntro;apply H7|].
+            iClear "Hw HSVInterp HVPC".
+            rewrite fixpoint_interp1_eq /=.
+            destruct Hp as [-> | [-> | [-> _] ] ]; try iFrame "HVPC'". destruct x0; try done; iFrame "HVPC'". 
+        }
+        iIntros (v) "Hv". iIntros (Hhalted).
+        iDestruct ("Hv" $! Hhalted) as (r0 W') "(Hfull & Hregs & % & Hown & sts & Hr)".
+        iExists _,_. iFrame. iPureIntro. eapply related_sts_pub_priv_trans_world;eauto.
+    }
     { iApply wp_pure_step_later; auto. iNext. iApply wp_value; auto. iIntros; discriminate. }
-    Unshelve. all: eauto; try exact {[a:=x]}.
+    Unshelve. all: auto.
   Qed.
 
 End fundamental.
